proof/agp32_EX_Flags_CorrectScript.sml
@@ -1,0 +1,1244 @@
+open hardwarePreamble translatorTheory translatorLib arithmeticTheory wordsExtraTheory dep_rewrite blastLib bitstringSyntax fcpSyntax listSyntax wordsSyntax agp32StateTheory agp32EnvironmentTheory agp32ProcessorTheory ag32Theory ag32ExtraTheory ag32UtilitiesTheory agp32RelationTheory agp32UpdateTheory agp32InternalTheory agp32SpecialTheory agp32_EX_CorrectTheory;
+
+(* correctness of EX stage flags with respect to the ISA *)
+val _ = new_theory "agp32_EX_Flags_Correct";
+
+val _ = prefer_num ();
+val _ = guess_lengths ();
+
+
+(** lemma **)
+Theorem overflow_rewrite[local]:
+  !x y.
+    w2i x + w2i y <> w2i (x + y) <=>
+    (word_msb x <=> word_msb y) /\ (word_msb x <> word_msb (x + y))
+Proof
+  METIS_TAC [integer_wordTheory.overflow]
+QED
+
+Theorem sub_overflow_rewrite[local]:
+  !x y.
+    w2i x - w2i y <> w2i (x - y) <=>
+    (word_msb x <> word_msb y) /\ (word_msb x <> word_msb (x - y))
+Proof
+  METIS_TAC [integer_wordTheory.sub_overflow]
+QED
+
+(** when EX is NONE, the EX_carry_flag and EX_overflow_flag are unchanged **)
+Theorem agp32_Rel_EX_NONE_flags_unchanged:
+  !fext fbits a t I.
+    is_sch I (agp32 fext fbits) a ==>
+    Rel I (fext t) (agp32 fext fbits (t-1)) (agp32 fext fbits t) a t ==>
+    I (3,SUC t) = NONE ==>
+    ((agp32 fext fbits (SUC t)).EX.EX_carry_flag = (agp32 fext fbits t).EX.EX_carry_flag) /\
+    ((agp32 fext fbits (SUC t)).EX.EX_overflow_flag = (agp32 fext fbits t).EX.EX_overflow_flag)
+Proof
+  rpt gen_tac >> rpt disch_tac >>
+  Q.ABBREV_TAC `s = agp32 fext fbits t` >>
+  Q.ABBREV_TAC `s' = procs [agp32_next_state;WB_pipeline;MEM_pipeline;EX_pipeline;
+                            REG_write;ID_pipeline;IF_PC_update;Acc_compute] (fext t) s s` >>
+  Q.ABBREV_TAC `s'' = procs [IF_instr_update;ID_opc_func_update;ID_imm_update;ID_data_update;
+                             ID_data_check_update;EX_ctrl_update;EX_ALU_input_imm_update] (fext (SUC t)) s' s'` >>
+  `((agp32 fext fbits (SUC t)).EX.EX_carry_flag =
+    (EX_ALU_update (fext (SUC t)) s' s'').EX.EX_carry_flag) /\
+  ((agp32 fext fbits (SUC t)).EX.EX_overflow_flag =
+   (EX_ALU_update (fext (SUC t)) s' s'').EX.EX_overflow_flag)`
+    by fs [agp32_EX_ALU_items_updated_by_EX_ALU_update] >>
+  `(s''.ID.ID_EX_write_enable = s.ID.ID_EX_write_enable) /\
+  (s''.EX.EX_overflow_flag = s.EX.EX_overflow_flag) /\
+  (s''.EX.EX_carry_flag = s.EX.EX_carry_flag)`
+    by METIS_TAC [agp32_same_items_until_EX_ALU_update,Abbr `s`,Abbr `s'`,Abbr `s''`] >>
+  `(s''.EX.EX_ALU_input1 = (agp32 fext fbits (SUC t)).EX.EX_ALU_input1) /\
+  (s''.EX.EX_ALU_input2 = (agp32 fext fbits (SUC t)).EX.EX_ALU_input2) /\
+  (s''.EX.EX_func = (agp32 fext fbits (SUC t)).EX.EX_func) /\
+  (s''.EX.EX_opc = (agp32 fext fbits (SUC t)).EX.EX_opc)`
+    by METIS_TAC [agp32_same_EX_ALU_input_until_ALU_update,agp32_same_EX_opc_func_until_ALU_update,
+                  Abbr `s`,Abbr `s'`,Abbr `s''`] >>
+  Cases_on `enable_stg 3 (agp32 fext fbits t)` >-
+   (`s''.ID.ID_EX_write_enable` by fs [enable_stg_def,Abbr `s`] >>
+    `((agp32 fext fbits (SUC t)).EX.EX_opc = 16w) \/ ((agp32 fext fbits (SUC t)).EX.EX_opc = 15w)`
+      by METIS_TAC [EX_instr_index_NONE_opc_flush] >>
+    `(s''.EX.EX_func = 9w) \/ (s''.EX.EX_func = 12w) \/ (s''.EX.EX_func = 13w) \/
+    (s''.EX.EX_func = 14w) \/ (s''.EX.EX_func = 15w)`
+      by fs [agp32_EX_opc_implies_EX_func] >>
+    fs [EX_ALU_update_def]) >>
+  `~s''.ID.ID_EX_write_enable` by fs [enable_stg_def,Abbr `s`] >>
+  fs [EX_ALU_update_def]
+QED
+
+
+(** EX_carry_flag **)
+Theorem agp32_Rel_ag32_EX_ALU_carry_flag_correct:
+  !fext fbits a t I.
+    is_sch I (agp32 fext fbits) a ==>
+    Rel I (fext t) (agp32 fext fbits (t-1)) (agp32 fext fbits t) a t ==>
+    I (3,SUC t) <> NONE ==>
+    (agp32 fext fbits (SUC t)).EX.EX_carry_flag = (FUNPOW Next (THE (I (3,SUC t))) a).CarryFlag
+Proof
+  rw [] >> Q.ABBREV_TAC `s = agp32 fext fbits t` >>
+  Q.ABBREV_TAC `s' = procs [agp32_next_state;WB_pipeline;MEM_pipeline;EX_pipeline;
+                            REG_write;ID_pipeline;IF_PC_update;Acc_compute] (fext t) s s` >>
+  Q.ABBREV_TAC `s'' = procs [IF_instr_update;ID_opc_func_update;ID_imm_update;ID_data_update;
+                             ID_data_check_update;EX_ctrl_update;EX_ALU_input_imm_update] (fext (SUC t)) s' s'` >>
+  `(agp32 fext fbits (SUC t)).EX.EX_carry_flag = (EX_ALU_update (fext (SUC t)) s' s'').EX.EX_carry_flag`
+    by fs [agp32_EX_ALU_items_updated_by_EX_ALU_update] >>
+  `(s''.ID.ID_EX_write_enable = s.ID.ID_EX_write_enable) /\
+  (s''.EX.EX_overflow_flag = s.EX.EX_overflow_flag) /\
+  (s''.EX.EX_carry_flag = s.EX.EX_carry_flag) /\
+  (s''.EX.EX_ALU_res = s.EX.EX_ALU_res)`
+    by METIS_TAC [agp32_same_items_until_EX_ALU_update,Abbr `s`,Abbr `s'`,Abbr `s''`] >>
+  `(s''.EX.EX_ALU_input1 = (agp32 fext fbits (SUC t)).EX.EX_ALU_input1) /\
+  (s''.EX.EX_ALU_input2 = (agp32 fext fbits (SUC t)).EX.EX_ALU_input2) /\
+  (s''.EX.EX_func = (agp32 fext fbits (SUC t)).EX.EX_func) /\
+  (s''.EX.EX_opc = (agp32 fext fbits (SUC t)).EX.EX_opc)`
+    by METIS_TAC [agp32_same_EX_ALU_input_until_ALU_update,agp32_same_EX_opc_func_until_ALU_update,
+                  Abbr `s`,Abbr `s'`,Abbr `s''`] >>
+  Cases_on `enable_stg 3 (agp32 fext fbits t)` >-
+   (`s''.ID.ID_EX_write_enable` by fs [enable_stg_def,Abbr `s`] >>
+    `s''.EX.EX_func = func (FUNPOW Next (THE (I' (3,SUC t)) − 1) a)`
+      by fs [is_sch_def,agp32_Rel_ag32_EX_func_correct] >>
+    `s''.EX.EX_opc = opc (FUNPOW Next (THE (I' (3,SUC t)) − 1) a)`
+      by fs [is_sch_def,agp32_Rel_ag32_EX_opc_correct] >>
+    `s''.EX.EX_ALU_input1 = ALU_input1 (FUNPOW Next (THE (I' (3,SUC t)) − 1) a)`
+      by fs [is_sch_def,agp32_Rel_ag32_EX_ALU_input1_correct] >>
+    `s''.EX.EX_ALU_input2 = ALU_input2 (FUNPOW Next (THE (I' (3,SUC t)) − 1) a)`
+      by fs [is_sch_def,agp32_Rel_ag32_EX_ALU_input2_correct] >>
+    Cases_on `I' (3,t) <> NONE` >-
+     (`THE (I' (3,SUC t)) = SUC (THE (I' (3,t)))`
+        by METIS_TAC [EX_instr_index_t_SUC_t_enable,ADD1] >> fs [FUNPOW_SUC] >>
+      Q.ABBREV_TAC `ai = FUNPOW Next (THE (I' (3,t))) a` >>
+      rw [Next_def,GSYM word_at_addr_def,GSYM align_addr_def] >>
+      Cases_on `Decode (word_at_addr ai.MEM (align_addr ai.PC))` >-
+       (PairCases_on `p` >> rw [Run_def,dfn'Accelerator_def,incPC_def] >>
+        `opc ai = 8w` by fs [ag32_Decode_Acc_opc_8w] >>
+        `(s''.EX.EX_func = 9w) \/ (s''.EX.EX_func = 12w) \/ (s''.EX.EX_func = 13w) \/
+        (s''.EX.EX_func = 14w) \/ (s''.EX.EX_func = 15w)`
+          by fs [agp32_EX_opc_implies_EX_func] >>
+        fs [EX_ALU_update_def,Rel_def]) >-
+       (rw [Run_def,dfn'In_def,incPC_def] >>
+        `opc ai = 7w` by fs [ag32_Decode_In_opc_7w] >>
+        `(s''.EX.EX_func = 9w) \/ (s''.EX.EX_func = 12w) \/ (s''.EX.EX_func = 13w) \/
+        (s''.EX.EX_func = 14w) \/ (s''.EX.EX_func = 15w)`
+          by fs [agp32_EX_opc_implies_EX_func] >>
+        fs [EX_ALU_update_def,Rel_def]) >-
+       (rw [Run_def,dfn'Interrupt_def,incPC_def] >>
+        `opc ai = 12w` by fs [ag32_Decode_Interrupt_opc_12w] >>
+        `(s''.EX.EX_func = 9w) \/ (s''.EX.EX_func = 12w) \/ (s''.EX.EX_func = 13w) \/
+        (s''.EX.EX_func = 14w) \/ (s''.EX.EX_func = 15w)`
+          by fs [agp32_EX_opc_implies_EX_func] >>
+        fs [EX_ALU_update_def,Rel_def]) >-
+       (PairCases_on `p` >> rw [Run_def,dfn'Jump_def] >>
+        `opc ai = 9w` by fs [ag32_Decode_Jump_opc_9w] >>
+        pairarg_tac >> fs [] >>
+        Cases_on `p0 = fAdd` >-
+         (fs [ALU_def] >> rw [] >>
+          `func ai = 0w` by fs [ag32_Decode_Jump_fAdd_func_0w] >> fs [] >>
+          rw [EX_ALU_update_def,ALU_correct_carry_lem,WORD_LS,word_add_def,w2n_w2w] >>
+          fs [ALU_input1_def,ALU_input2_def] >>
+          `dataA ai = ri2word p2 ai` by fs [ag32_Decode_Jump_dataA] >>
+          rw [] >> METIS_TAC [w2n_add_MOD_itself]) >>
+        Cases_on `p0 = fAddWithCarry` >-
+         (fs [ALU_def] >> rw [] >>
+          `func ai = 1w` by fs [ag32_Decode_Jump_fAddWithCarry_func_1w] >> fs [] >>
+          rw [EX_ALU_update_def,ALU_correct_carry_lem,WORD_LS,word_add_def,w2n_w2w] >>
+          fs [ALU_input1_def,ALU_input2_def] >>
+          `dataA ai = ri2word p2 ai` by fs [ag32_Decode_Jump_dataA] >-
+           (`s.EX.EX_carry_flag` by fs [Rel_def] >>
+            rw [v2w_single_1w,ALU_correct_v2w_carry33_lem] >>
+            METIS_TAC [w2n_add_MOD_itself_1]) >>
+          `~s.EX.EX_carry_flag` by fs [Rel_def] >>
+          rw [v2w_single_0w,ALU_correct_v2w_carry33_lem] >>
+          METIS_TAC [w2n_add_MOD_itself]) >>
+        fs [] >> rename1 `(v,ai')` >>
+        `ai'.CarryFlag = ai.CarryFlag` by (fs [ALU_def] >> Cases_on `p0` >> fs [] >> rw []) >>
+        `(func ai <> 0w) /\ (func ai <> 1w)` by fs [ag32_Decode_Jump_func_not_0w_1w] >>
+        fs [EX_ALU_update_def,Rel_def] >>
+        Cases_on_word_value `(agp32 fext fbits (SUC t)).EX.EX_func` >> fs []) >-
+       (PairCases_on `p` >> rw [Run_def,dfn'JumpIfNotZero_def] >>
+        `opc ai = 11w` by fs [ag32_Decode_JumpIfNotZero_opc_11w] >>
+        pairarg_tac >> fs [] >>
+        Cases_on `p0 = fAdd` >-
+         (fs [ALU_def] >> rw [] >>
+          `func ai = 0w` by fs [ag32_Decode_JumpIfNotZero_fAdd_func_0w] >> fs [] >>
+          rw [EX_ALU_update_def,ALU_correct_carry_lem,WORD_LS,word_add_def,w2n_w2w] >>
+          fs [ALU_input1_def,ALU_input2_def] >>
+          `(dataA ai = ri2word p2 ai) /\ (dataB ai = ri2word p3 ai)`
+            by fs [ag32_Decode_JumpIfNotZero_dataA,ag32_Decode_JumpIfNotZero_dataB] >>
+          rw [incPC_def] >> METIS_TAC [w2n_add_MOD_itself]) >>
+        Cases_on `p0 = fAddWithCarry` >-
+         (fs [ALU_def] >> rw [] >>
+          `func ai = 1w` by fs [ag32_Decode_JumpIfNotZero_fAddWithCarry_func_1w] >> fs [] >>
+          rw [EX_ALU_update_def,ALU_correct_carry_lem,WORD_LS,word_add_def,w2n_w2w] >>
+          fs [ALU_input1_def,ALU_input2_def] >>
+          `(dataA ai = ri2word p2 ai) /\ (dataB ai = ri2word p3 ai)`
+            by fs [ag32_Decode_JumpIfNotZero_dataA,ag32_Decode_JumpIfNotZero_dataB] >-
+           (`s.EX.EX_carry_flag` by fs [Rel_def] >>
+            rw [v2w_single_1w,ALU_correct_v2w_carry33_lem] >>
+            METIS_TAC [w2n_add_MOD_itself_1]) >-
+           (`~s.EX.EX_carry_flag` by fs [Rel_def] >>
+            rw [v2w_single_0w,ALU_correct_v2w_carry33_lem] >>
+            METIS_TAC [w2n_add_MOD_itself]) >-
+           (`s.EX.EX_carry_flag` by fs [Rel_def] >>
+            rw [v2w_single_1w,ALU_correct_v2w_carry33_lem,incPC_def] >>
+            METIS_TAC [w2n_add_MOD_itself_1]) >>
+          `~s.EX.EX_carry_flag` by fs [Rel_def] >>
+          rw [v2w_single_0w,ALU_correct_v2w_carry33_lem,incPC_def] >>
+          METIS_TAC [w2n_add_MOD_itself]) >>
+        fs [] >> rename1 `(v,ai')` >>
+        `ai'.CarryFlag = ai.CarryFlag` by (fs [ALU_def] >> Cases_on `p0` >> fs [] >> rw []) >>
+        `(func ai <> 0w) /\ (func ai <> 1w)` by fs [ag32_Decode_JumpIfNotZero_func_not_0w_1w] >>
+        Cases_on `v` >> rw [incPC_def] >>
+        fs [EX_ALU_update_def,Rel_def,incPC_def] >>
+        Cases_on_word_value `(agp32 fext fbits (SUC t)).EX.EX_func` >> fs []) >-
+       (PairCases_on `p` >> rw [Run_def,dfn'JumpIfZero_def] >>
+        `opc ai = 10w` by fs [ag32_Decode_JumpIfZero_opc_10w] >>
+        pairarg_tac >> fs [] >>
+        Cases_on `p0 = fAdd` >-
+         (fs [ALU_def] >> rw [] >>
+          `func ai = 0w` by fs [ag32_Decode_JumpIfZero_fAdd_func_0w] >> fs [] >>
+          rw [EX_ALU_update_def,ALU_correct_carry_lem,WORD_LS,word_add_def,w2n_w2w] >>
+          fs [ALU_input1_def,ALU_input2_def] >>
+          `(dataA ai = ri2word p2 ai) /\ (dataB ai = ri2word p3 ai)`
+            by fs [ag32_Decode_JumpIfZero_dataA,ag32_Decode_JumpIfZero_dataB] >>
+          rw [incPC_def] >> METIS_TAC [w2n_add_MOD_itself]) >>
+        Cases_on `p0 = fAddWithCarry` >-
+         (fs [ALU_def] >> rw [] >>
+          `func ai = 1w` by fs [ag32_Decode_JumpIfZero_fAddWithCarry_func_1w] >> fs [] >>
+          rw [EX_ALU_update_def,ALU_correct_carry_lem,WORD_LS,word_add_def,w2n_w2w] >>
+          fs [ALU_input1_def,ALU_input2_def] >>
+          `(dataA ai = ri2word p2 ai) /\ (dataB ai = ri2word p3 ai)`
+            by fs [ag32_Decode_JumpIfZero_dataA,ag32_Decode_JumpIfZero_dataB] >-
+           (`s.EX.EX_carry_flag` by fs [Rel_def] >>
+            rw [v2w_single_1w,ALU_correct_v2w_carry33_lem] >>
+            METIS_TAC [w2n_add_MOD_itself_1]) >-
+           (`~s.EX.EX_carry_flag` by fs [Rel_def] >>
+            rw [v2w_single_0w,ALU_correct_v2w_carry33_lem] >>
+            METIS_TAC [w2n_add_MOD_itself]) >-
+           (`s.EX.EX_carry_flag` by fs [Rel_def] >>
+            rw [v2w_single_1w,ALU_correct_v2w_carry33_lem,incPC_def] >>
+            METIS_TAC [w2n_add_MOD_itself_1]) >>
+          `~s.EX.EX_carry_flag` by fs [Rel_def] >>
+          rw [v2w_single_0w,ALU_correct_v2w_carry33_lem,incPC_def] >>
+          METIS_TAC [w2n_add_MOD_itself]) >>
+        fs [] >> rename1 `(v,ai')` >>
+        `ai'.CarryFlag = ai.CarryFlag` by (fs [ALU_def] >> Cases_on `p0` >> fs [] >> rw []) >>
+        `(func ai <> 0w) /\ (func ai <> 1w)` by fs [ag32_Decode_JumpIfZero_func_not_0w_1w] >>
+        Cases_on `v` >> rw [incPC_def] >>
+        fs [EX_ALU_update_def,Rel_def,incPC_def] >>
+        Cases_on_word_value `(agp32 fext fbits (SUC t)).EX.EX_func` >> fs []) >-
+       (PairCases_on `p` >> rw [Run_def,dfn'LoadConstant_def,incPC_def] >>
+        `opc ai = 13w` by fs [ag32_Decode_LoadConstant_opc_13w] >>
+        `(s''.EX.EX_func = 9w) \/ (s''.EX.EX_func = 12w) \/ (s''.EX.EX_func = 13w) \/
+        (s''.EX.EX_func = 14w) \/ (s''.EX.EX_func = 15w)`
+          by fs [agp32_EX_opc_implies_EX_func] >>
+        fs [EX_ALU_update_def,Rel_def]) >-
+       (PairCases_on `p` >> rw [Run_def,dfn'LoadMEM_def,incPC_def] >>
+        `opc ai = 4w` by fs [ag32_Decode_LoadMEM_opc_4w] >>
+        `(s''.EX.EX_func = 9w) \/ (s''.EX.EX_func = 12w) \/ (s''.EX.EX_func = 13w) \/
+        (s''.EX.EX_func = 14w) \/ (s''.EX.EX_func = 15w)`
+          by fs [agp32_EX_opc_implies_EX_func] >>
+        fs [EX_ALU_update_def,Rel_def]) >-
+       (PairCases_on `p` >> rw [Run_def,dfn'LoadMEMByte_def,incPC_def] >>
+        `opc ai = 5w` by fs [ag32_Decode_LoadMEMByte_opc_5w] >>
+        `(s''.EX.EX_func = 9w) \/ (s''.EX.EX_func = 12w) \/ (s''.EX.EX_func = 13w) \/
+        (s''.EX.EX_func = 14w) \/ (s''.EX.EX_func = 15w)`
+          by fs [agp32_EX_opc_implies_EX_func] >>
+        fs [EX_ALU_update_def,Rel_def]) >-
+       (PairCases_on `p` >> rw [Run_def,dfn'LoadUpperConstant_def,incPC_def] >>
+        `opc ai = 14w` by fs [ag32_Decode_LoadUpperConstant_opc_14w] >>
+        `(s''.EX.EX_func = 9w) \/ (s''.EX.EX_func = 12w) \/ (s''.EX.EX_func = 13w) \/
+        (s''.EX.EX_func = 14w) \/ (s''.EX.EX_func = 15w)`
+          by fs [agp32_EX_opc_implies_EX_func] >>
+        fs [EX_ALU_update_def,Rel_def]) >-
+       (PairCases_on `p` >> rw [Run_def,dfn'Normal_def,norm_def,incPC_def] >>
+        `opc ai = 0w` by fs [ag32_Decode_Normal_opc_0w] >>
+        pairarg_tac >> fs [] >>
+        Cases_on `p0 = fAdd` >-
+         (fs [ALU_def] >> rw [] >>
+          `func ai = 0w` by fs [ag32_Decode_Normal_fAdd_func_0w] >> fs [] >>
+          rw [EX_ALU_update_def,ALU_correct_carry_lem,WORD_LS,word_add_def,w2n_w2w] >>
+          fs [ALU_input1_def,ALU_input2_def] >>
+          `(dataA ai = ri2word p2 ai) /\ (dataB ai = ri2word p3 ai)`
+            by fs [ag32_Decode_Normal_dataA,ag32_Decode_Normal_dataB] >>
+          rw [] >> METIS_TAC [w2n_add_MOD_itself]) >>
+        Cases_on `p0 = fAddWithCarry` >-
+         (fs [ALU_def] >> rw [] >>
+          `func ai = 1w` by fs [ag32_Decode_Normal_fAddWithCarry_func_1w] >> fs [] >>
+          rw [EX_ALU_update_def,ALU_correct_carry_lem,WORD_LS,word_add_def,w2n_w2w] >>
+          fs [ALU_input1_def,ALU_input2_def] >>
+          `(dataA ai = ri2word p2 ai) /\ (dataB ai = ri2word p3 ai)`
+            by fs [ag32_Decode_Normal_dataA,ag32_Decode_Normal_dataB] >-
+           (`s.EX.EX_carry_flag` by fs [Rel_def] >>
+            rw [v2w_single_1w,ALU_correct_v2w_carry33_lem] >>
+            METIS_TAC [w2n_add_MOD_itself_1]) >>
+          `~s.EX.EX_carry_flag` by fs [Rel_def] >>
+          rw [v2w_single_0w,ALU_correct_v2w_carry33_lem] >>
+          METIS_TAC [w2n_add_MOD_itself]) >>
+        fs [] >> rename1 `(v,ai')` >>
+        `ai'.CarryFlag = ai.CarryFlag` by (fs [ALU_def] >> Cases_on `p0` >> fs [] >> rw []) >>
+        `(func ai <> 0w) /\ (func ai <> 1w)` by fs [ag32_Decode_Normal_func_not_0w_1w] >>
+        fs [EX_ALU_update_def,Rel_def] >>
+        Cases_on_word_value `(agp32 fext fbits (SUC t)).EX.EX_func` >> fs []) >-
+       (PairCases_on `p` >> rw [Run_def,dfn'Out_def,norm_def,incPC_def] >>
+        `opc ai = 6w` by fs [ag32_Decode_Out_opc_6w] >>
+        pairarg_tac >> fs [] >>
+        Cases_on `p0 = fAdd` >-
+         (fs [ALU_def] >> rw [] >>
+          `func ai = 0w` by fs [ag32_Decode_Out_fAdd_func_0w] >> fs [] >>
+          rw [EX_ALU_update_def,ALU_correct_carry_lem,WORD_LS,word_add_def,w2n_w2w] >>
+          fs [ALU_input1_def,ALU_input2_def] >>
+          `(dataA ai = ri2word p2 ai) /\ (dataB ai = ri2word p3 ai)`
+            by fs [ag32_Decode_Out_dataA,ag32_Decode_Out_dataB] >>
+          rw [] >> METIS_TAC [w2n_add_MOD_itself]) >>
+        Cases_on `p0 = fAddWithCarry` >-
+         (fs [ALU_def] >> rw [] >>
+          `func ai = 1w` by fs [ag32_Decode_Out_fAddWithCarry_func_1w] >> fs [] >>
+          rw [EX_ALU_update_def,ALU_correct_carry_lem,WORD_LS,word_add_def,w2n_w2w] >>
+          fs [ALU_input1_def,ALU_input2_def] >>
+          `(dataA ai = ri2word p2 ai) /\ (dataB ai = ri2word p3 ai)`
+            by fs [ag32_Decode_Out_dataA,ag32_Decode_Out_dataB] >-
+           (`s.EX.EX_carry_flag` by fs [Rel_def] >>
+            rw [v2w_single_1w,ALU_correct_v2w_carry33_lem] >>
+            METIS_TAC [w2n_add_MOD_itself_1]) >>
+          `~s.EX.EX_carry_flag` by fs [Rel_def] >>
+          rw [v2w_single_0w,ALU_correct_v2w_carry33_lem] >>
+          METIS_TAC [w2n_add_MOD_itself]) >>
+        fs [] >> rename1 `(v,ai')` >>
+        `ai'.CarryFlag = ai.CarryFlag` by (fs [ALU_def] >> Cases_on `p0` >> fs [] >> rw []) >>
+        `(func ai <> 0w) /\ (func ai <> 1w)` by fs [ag32_Decode_Out_func_not_0w_1w] >>
+        fs [EX_ALU_update_def,Rel_def] >>
+        Cases_on_word_value `(agp32 fext fbits (SUC t)).EX.EX_func` >> fs []) >-
+       (rw [Run_def] >>
+        `opc ai = 15w` by fs [ag32_Decode_ReservedInstr_opc_15w] >>
+        `(s''.EX.EX_func = 9w) \/ (s''.EX.EX_func = 12w) \/ (s''.EX.EX_func = 13w) \/
+        (s''.EX.EX_func = 14w) \/ (s''.EX.EX_func = 15w)`
+          by fs [agp32_EX_opc_implies_EX_func] >>
+        fs [EX_ALU_update_def,Rel_def]) >-
+       (PairCases_on `p` >> rw [Run_def,dfn'Shift_def,incPC_def] >>
+        `opc ai = 1w` by fs [ag32_Decode_Shift_opc_1w] >>
+        `(s''.EX.EX_func = 9w) \/ (s''.EX.EX_func = 12w) \/ (s''.EX.EX_func = 13w) \/
+        (s''.EX.EX_func = 14w) \/ (s''.EX.EX_func = 15w)`
+          by fs [agp32_EX_opc_implies_EX_func] >>
+        fs [EX_ALU_update_def,Rel_def]) >-
+       (PairCases_on `p` >> rw [Run_def,dfn'StoreMEM_def,incPC_def] >>
+        `opc ai = 2w` by fs [ag32_Decode_StoreMEM_opc_2w] >>
+        `(s''.EX.EX_func = 9w) \/ (s''.EX.EX_func = 12w) \/ (s''.EX.EX_func = 13w) \/
+        (s''.EX.EX_func = 14w) \/ (s''.EX.EX_func = 15w)`
+          by fs [agp32_EX_opc_implies_EX_func] >>
+        fs [EX_ALU_update_def,Rel_def]) >>
+      PairCases_on `p` >> rw [Run_def,dfn'StoreMEMByte_def,incPC_def] >>
+      `opc ai = 3w` by fs [ag32_Decode_StoreMEMByte_opc_3w] >>
+      `(s''.EX.EX_func = 9w) \/ (s''.EX.EX_func = 12w) \/ (s''.EX.EX_func = 13w) \/
+      (s''.EX.EX_func = 14w) \/ (s''.EX.EX_func = 15w)`
+        by fs [agp32_EX_opc_implies_EX_func] >>
+      fs [EX_ALU_update_def,Rel_def]) >>
+    subgoal `I' (3,SUC t) = I' (2,t)` >-
+     (fs [is_sch_def,is_sch_execute_def] >>
+      Cases_on `isJump_hw_op (agp32 fext fbits t)` >>
+      Cases_on `reg_data_hazard (agp32 fext fbits t)` >>
+      METIS_TAC []) >> fs [] >>
+    `THE (I' (2,t)) = SUC (THE (I' (2,t)) - 1)`
+      by (Cases_on `THE (I' (2,t))` >- METIS_TAC [ID_instr_index_not_0] >> fs []) >>
+    `(FUNPOW Next (THE (I' (2,t))) a).CarryFlag =
+    (FUNPOW Next (SUC (THE (I' (2,t)) - 1)) a).CarryFlag` by METIS_TAC [] >>       
+    fs [FUNPOW_SUC] >>
+    Q.ABBREV_TAC `ai = FUNPOW Next (THE (I' (2,t)) - 1) a` >>
+    rw [Next_def,GSYM word_at_addr_def,GSYM align_addr_def] >>
+    Cases_on `Decode (word_at_addr ai.MEM (align_addr ai.PC))` >-
+     (PairCases_on `p` >> rw [Run_def,dfn'Accelerator_def,incPC_def] >>
+      `opc ai = 8w` by fs [ag32_Decode_Acc_opc_8w] >>
+      `(s''.EX.EX_func = 9w) \/ (s''.EX.EX_func = 12w) \/ (s''.EX.EX_func = 13w) \/
+      (s''.EX.EX_func = 14w) \/ (s''.EX.EX_func = 15w)`         
+        by fs [agp32_EX_opc_implies_EX_func] >>
+      fs [EX_ALU_update_def,Rel_def]) >-
+     (rw [Run_def,dfn'In_def,incPC_def] >>
+      `opc ai = 7w` by fs [ag32_Decode_In_opc_7w] >>
+      `(s''.EX.EX_func = 9w) \/ (s''.EX.EX_func = 12w) \/ (s''.EX.EX_func = 13w) \/
+      (s''.EX.EX_func = 14w) \/ (s''.EX.EX_func = 15w)`
+        by fs [agp32_EX_opc_implies_EX_func] >>
+      fs [EX_ALU_update_def,Rel_def]) >-
+     (rw [Run_def,dfn'Interrupt_def,incPC_def] >>
+      `opc ai = 12w` by fs [ag32_Decode_Interrupt_opc_12w] >>
+      `(s''.EX.EX_func = 9w) \/ (s''.EX.EX_func = 12w) \/ (s''.EX.EX_func = 13w) \/
+      (s''.EX.EX_func = 14w) \/ (s''.EX.EX_func = 15w)`
+        by fs [agp32_EX_opc_implies_EX_func] >>
+      fs [EX_ALU_update_def,Rel_def]) >-
+     (PairCases_on `p` >> rw [Run_def,dfn'Jump_def] >>
+      `opc ai = 9w` by fs [ag32_Decode_Jump_opc_9w] >>
+      pairarg_tac >> fs [] >>
+      Cases_on `p0 = fAdd` >-
+       (fs [ALU_def] >> rw [] >>
+        `func ai = 0w` by fs [ag32_Decode_Jump_fAdd_func_0w] >> fs [] >>
+        rw [EX_ALU_update_def,ALU_correct_carry_lem,WORD_LS,word_add_def,w2n_w2w] >>
+        fs [ALU_input1_def,ALU_input2_def] >>
+        `dataA ai = ri2word p2 ai` by fs [ag32_Decode_Jump_dataA] >>
+        rw [] >> METIS_TAC [w2n_add_MOD_itself]) >>
+      Cases_on `p0 = fAddWithCarry` >-
+       (fs [ALU_def] >> rw [] >>
+        `func ai = 1w` by fs [ag32_Decode_Jump_fAddWithCarry_func_1w] >> fs [] >>
+        rw [EX_ALU_update_def,ALU_correct_carry_lem,WORD_LS,word_add_def,w2n_w2w] >>
+        fs [ALU_input1_def,ALU_input2_def] >>
+        `dataA ai = ri2word p2 ai` by fs [ag32_Decode_Jump_dataA] >-
+         (`s.EX.EX_carry_flag` by fs [Rel_def] >>
+          rw [v2w_single_1w,ALU_correct_v2w_carry33_lem] >>
+          METIS_TAC [w2n_add_MOD_itself_1]) >>
+        `~s.EX.EX_carry_flag` by fs [Rel_def] >>
+        rw [v2w_single_0w,ALU_correct_v2w_carry33_lem] >>
+        METIS_TAC [w2n_add_MOD_itself]) >>
+      fs [] >> rename1 `(v,ai')` >>
+      `ai'.CarryFlag = ai.CarryFlag` by (fs [ALU_def] >> Cases_on `p0` >> fs [] >> rw []) >>
+      `(func ai <> 0w) /\ (func ai <> 1w)` by fs [ag32_Decode_Jump_func_not_0w_1w] >>
+      fs [EX_ALU_update_def,Rel_def] >>
+      Cases_on_word_value `(agp32 fext fbits (SUC t)).EX.EX_func` >> fs []) >-
+     (PairCases_on `p` >> rw [Run_def,dfn'JumpIfNotZero_def] >>
+      `opc ai = 11w` by fs [ag32_Decode_JumpIfNotZero_opc_11w] >>
+      pairarg_tac >> fs [] >>
+      Cases_on `p0 = fAdd` >-
+       (fs [ALU_def] >> rw [] >>
+        `func ai = 0w` by fs [ag32_Decode_JumpIfNotZero_fAdd_func_0w] >> fs [] >>
+        rw [EX_ALU_update_def,ALU_correct_carry_lem,WORD_LS,word_add_def,w2n_w2w] >>
+        fs [ALU_input1_def,ALU_input2_def] >>
+        `(dataA ai = ri2word p2 ai) /\ (dataB ai = ri2word p3 ai)`
+          by fs [ag32_Decode_JumpIfNotZero_dataA,ag32_Decode_JumpIfNotZero_dataB] >>
+        rw [incPC_def] >> METIS_TAC [w2n_add_MOD_itself]) >>
+      Cases_on `p0 = fAddWithCarry` >-
+       (fs [ALU_def] >> rw [] >>
+        `func ai = 1w` by fs [ag32_Decode_JumpIfNotZero_fAddWithCarry_func_1w] >> fs [] >>
+        rw [EX_ALU_update_def,ALU_correct_carry_lem,WORD_LS,word_add_def,w2n_w2w] >>
+        fs [ALU_input1_def,ALU_input2_def] >>
+        `(dataA ai = ri2word p2 ai) /\ (dataB ai = ri2word p3 ai)`
+          by fs [ag32_Decode_JumpIfNotZero_dataA,ag32_Decode_JumpIfNotZero_dataB] >-
+         (`s.EX.EX_carry_flag` by fs [Rel_def] >>
+          rw [v2w_single_1w,ALU_correct_v2w_carry33_lem] >>
+          METIS_TAC [w2n_add_MOD_itself_1]) >-
+         (`~s.EX.EX_carry_flag` by fs [Rel_def] >>
+          rw [v2w_single_0w,ALU_correct_v2w_carry33_lem] >>
+          METIS_TAC [w2n_add_MOD_itself]) >-
+         (`s.EX.EX_carry_flag` by fs [Rel_def] >>
+          rw [v2w_single_1w,ALU_correct_v2w_carry33_lem,incPC_def] >>
+          METIS_TAC [w2n_add_MOD_itself_1]) >>
+        `~s.EX.EX_carry_flag` by fs [Rel_def] >>
+        rw [v2w_single_0w,ALU_correct_v2w_carry33_lem,incPC_def] >>
+        METIS_TAC [w2n_add_MOD_itself]) >>
+      fs [] >> rename1 `(v,ai')` >>
+      `ai'.CarryFlag = ai.CarryFlag` by (fs [ALU_def] >> Cases_on `p0` >> fs [] >> rw []) >>
+      `(func ai <> 0w) /\ (func ai <> 1w)` by fs [ag32_Decode_JumpIfNotZero_func_not_0w_1w] >>
+      Cases_on `v` >> rw [incPC_def] >>
+      fs [EX_ALU_update_def,Rel_def,incPC_def] >>
+      Cases_on_word_value `(agp32 fext fbits (SUC t)).EX.EX_func` >> fs []) >-
+     (PairCases_on `p` >> rw [Run_def,dfn'JumpIfZero_def] >>
+      `opc ai = 10w` by fs [ag32_Decode_JumpIfZero_opc_10w] >>
+      pairarg_tac >> fs [] >>
+      Cases_on `p0 = fAdd` >-
+       (fs [ALU_def] >> rw [] >>
+        `func ai = 0w` by fs [ag32_Decode_JumpIfZero_fAdd_func_0w] >> fs [] >>
+        rw [EX_ALU_update_def,ALU_correct_carry_lem,WORD_LS,word_add_def,w2n_w2w] >>
+        fs [ALU_input1_def,ALU_input2_def] >>
+        `(dataA ai = ri2word p2 ai) /\ (dataB ai = ri2word p3 ai)`
+          by fs [ag32_Decode_JumpIfZero_dataA,ag32_Decode_JumpIfZero_dataB] >>
+        rw [incPC_def] >> METIS_TAC [w2n_add_MOD_itself]) >>
+      Cases_on `p0 = fAddWithCarry` >-
+       (fs [ALU_def] >> rw [] >>
+        `func ai = 1w` by fs [ag32_Decode_JumpIfZero_fAddWithCarry_func_1w] >> fs [] >>
+        rw [EX_ALU_update_def,ALU_correct_carry_lem,WORD_LS,word_add_def,w2n_w2w] >>
+        fs [ALU_input1_def,ALU_input2_def] >>
+        `(dataA ai = ri2word p2 ai) /\ (dataB ai = ri2word p3 ai)`
+          by fs [ag32_Decode_JumpIfZero_dataA,ag32_Decode_JumpIfZero_dataB] >-
+         (`s.EX.EX_carry_flag` by fs [Rel_def] >>
+          rw [v2w_single_1w,ALU_correct_v2w_carry33_lem] >>
+          METIS_TAC [w2n_add_MOD_itself_1]) >-
+         (`~s.EX.EX_carry_flag` by fs [Rel_def] >>
+          rw [v2w_single_0w,ALU_correct_v2w_carry33_lem] >>
+          METIS_TAC [w2n_add_MOD_itself]) >-
+         (`s.EX.EX_carry_flag` by fs [Rel_def] >>
+          rw [v2w_single_1w,ALU_correct_v2w_carry33_lem,incPC_def] >>
+          METIS_TAC [w2n_add_MOD_itself_1]) >>
+        `~s.EX.EX_carry_flag` by fs [Rel_def] >>
+        rw [v2w_single_0w,ALU_correct_v2w_carry33_lem,incPC_def] >>
+        METIS_TAC [w2n_add_MOD_itself]) >>
+      fs [] >> rename1 `(v,ai')` >>
+      `ai'.CarryFlag = ai.CarryFlag` by (fs [ALU_def] >> Cases_on `p0` >> fs [] >> rw []) >>
+      `(func ai <> 0w) /\ (func ai <> 1w)` by fs [ag32_Decode_JumpIfZero_func_not_0w_1w] >>
+      Cases_on `v` >> rw [incPC_def] >>
+      fs [EX_ALU_update_def,Rel_def,incPC_def] >>
+      Cases_on_word_value `(agp32 fext fbits (SUC t)).EX.EX_func` >> fs []) >-
+     (PairCases_on `p` >> rw [Run_def,dfn'LoadConstant_def,incPC_def] >>
+      `opc ai = 13w` by fs [ag32_Decode_LoadConstant_opc_13w] >>
+      `(s''.EX.EX_func = 9w) \/ (s''.EX.EX_func = 12w) \/ (s''.EX.EX_func = 13w) \/
+      (s''.EX.EX_func = 14w) \/ (s''.EX.EX_func = 15w)`
+        by fs [agp32_EX_opc_implies_EX_func] >>
+      fs [EX_ALU_update_def,Rel_def]) >-
+     (PairCases_on `p` >> rw [Run_def,dfn'LoadMEM_def,incPC_def] >>
+      `opc ai = 4w` by fs [ag32_Decode_LoadMEM_opc_4w] >>
+      `(s''.EX.EX_func = 9w) \/ (s''.EX.EX_func = 12w) \/ (s''.EX.EX_func = 13w) \/
+      (s''.EX.EX_func = 14w) \/ (s''.EX.EX_func = 15w)`
+        by fs [agp32_EX_opc_implies_EX_func] >>
+      fs [EX_ALU_update_def,Rel_def]) >-
+     (PairCases_on `p` >> rw [Run_def,dfn'LoadMEMByte_def,incPC_def] >>
+      `opc ai = 5w` by fs [ag32_Decode_LoadMEMByte_opc_5w] >>
+      `(s''.EX.EX_func = 9w) \/ (s''.EX.EX_func = 12w) \/ (s''.EX.EX_func = 13w) \/
+      (s''.EX.EX_func = 14w) \/ (s''.EX.EX_func = 15w)`
+        by fs [agp32_EX_opc_implies_EX_func] >>
+      fs [EX_ALU_update_def,Rel_def]) >-
+     (PairCases_on `p` >> rw [Run_def,dfn'LoadUpperConstant_def,incPC_def] >>
+      `opc ai = 14w` by fs [ag32_Decode_LoadUpperConstant_opc_14w] >>
+      `(s''.EX.EX_func = 9w) \/ (s''.EX.EX_func = 12w) \/ (s''.EX.EX_func = 13w) \/
+      (s''.EX.EX_func = 14w) \/ (s''.EX.EX_func = 15w)`
+        by fs [agp32_EX_opc_implies_EX_func] >>
+      fs [EX_ALU_update_def,Rel_def]) >-
+     (PairCases_on `p` >> rw [Run_def,dfn'Normal_def,norm_def,incPC_def] >>
+      `opc ai = 0w` by fs [ag32_Decode_Normal_opc_0w] >>
+      pairarg_tac >> fs [] >>
+      Cases_on `p0 = fAdd` >-
+       (fs [ALU_def] >> rw [] >>
+        `func ai = 0w` by fs [ag32_Decode_Normal_fAdd_func_0w] >> fs [] >>
+        rw [EX_ALU_update_def,ALU_correct_carry_lem,WORD_LS,word_add_def,w2n_w2w] >>
+        fs [ALU_input1_def,ALU_input2_def] >>
+        `(dataA ai = ri2word p2 ai) /\ (dataB ai = ri2word p3 ai)`
+          by fs [ag32_Decode_Normal_dataA,ag32_Decode_Normal_dataB] >>
+        rw [] >> METIS_TAC [w2n_add_MOD_itself]) >>
+      Cases_on `p0 = fAddWithCarry` >-
+       (fs [ALU_def] >> rw [] >>
+        `func ai = 1w` by fs [ag32_Decode_Normal_fAddWithCarry_func_1w] >> fs [] >>
+        rw [EX_ALU_update_def,ALU_correct_carry_lem,WORD_LS,word_add_def,w2n_w2w] >>
+        fs [ALU_input1_def,ALU_input2_def] >>
+        `(dataA ai = ri2word p2 ai) /\ (dataB ai = ri2word p3 ai)`
+          by fs [ag32_Decode_Normal_dataA,ag32_Decode_Normal_dataB] >-
+         (`s.EX.EX_carry_flag` by fs [Rel_def] >>
+          rw [v2w_single_1w,ALU_correct_v2w_carry33_lem] >>
+          METIS_TAC [w2n_add_MOD_itself_1]) >>
+        `~s.EX.EX_carry_flag` by fs [Rel_def] >>
+        rw [v2w_single_0w,ALU_correct_v2w_carry33_lem] >>
+        METIS_TAC [w2n_add_MOD_itself]) >>
+      fs [] >> rename1 `(v,ai')` >>
+      `ai'.CarryFlag = ai.CarryFlag` by (fs [ALU_def] >> Cases_on `p0` >> fs [] >> rw []) >>
+      `(func ai <> 0w) /\ (func ai <> 1w)` by fs [ag32_Decode_Normal_func_not_0w_1w] >>
+      fs [EX_ALU_update_def,Rel_def] >>
+      Cases_on_word_value `(agp32 fext fbits (SUC t)).EX.EX_func` >> fs []) >-
+     (PairCases_on `p` >> rw [Run_def,dfn'Out_def,norm_def,incPC_def] >>
+      `opc ai = 6w` by fs [ag32_Decode_Out_opc_6w] >>
+      pairarg_tac >> fs [] >>
+      Cases_on `p0 = fAdd` >-
+       (fs [ALU_def] >> rw [] >>
+        `func ai = 0w` by fs [ag32_Decode_Out_fAdd_func_0w] >> fs [] >>
+        rw [EX_ALU_update_def,ALU_correct_carry_lem,WORD_LS,word_add_def,w2n_w2w] >>
+        fs [ALU_input1_def,ALU_input2_def] >>
+        `(dataA ai = ri2word p2 ai) /\ (dataB ai = ri2word p3 ai)`
+          by fs [ag32_Decode_Out_dataA,ag32_Decode_Out_dataB] >>
+        rw [] >> METIS_TAC [w2n_add_MOD_itself]) >>
+      Cases_on `p0 = fAddWithCarry` >-
+       (fs [ALU_def] >> rw [] >>
+        `func ai = 1w` by fs [ag32_Decode_Out_fAddWithCarry_func_1w] >> fs [] >>
+        rw [EX_ALU_update_def,ALU_correct_carry_lem,WORD_LS,word_add_def,w2n_w2w] >>
+        fs [ALU_input1_def,ALU_input2_def] >>
+        `(dataA ai = ri2word p2 ai) /\ (dataB ai = ri2word p3 ai)`
+          by fs [ag32_Decode_Out_dataA,ag32_Decode_Out_dataB] >-
+         (`s.EX.EX_carry_flag` by fs [Rel_def] >>
+          rw [v2w_single_1w,ALU_correct_v2w_carry33_lem] >>
+          METIS_TAC [w2n_add_MOD_itself_1]) >>
+        `~s.EX.EX_carry_flag` by fs [Rel_def] >>
+        rw [v2w_single_0w,ALU_correct_v2w_carry33_lem] >>
+        METIS_TAC [w2n_add_MOD_itself]) >>
+      fs [] >> rename1 `(v,ai')` >>
+      `ai'.CarryFlag = ai.CarryFlag` by (fs [ALU_def] >> Cases_on `p0` >> fs [] >> rw []) >>
+      `(func ai <> 0w) /\ (func ai <> 1w)` by fs [ag32_Decode_Out_func_not_0w_1w] >>
+      fs [EX_ALU_update_def,Rel_def] >>
+      Cases_on_word_value `(agp32 fext fbits (SUC t)).EX.EX_func` >> fs []) >-
+     (rw [Run_def] >>
+      `opc ai = 15w` by fs [ag32_Decode_ReservedInstr_opc_15w] >>
+      `(s''.EX.EX_func = 9w) \/ (s''.EX.EX_func = 12w) \/ (s''.EX.EX_func = 13w) \/
+      (s''.EX.EX_func = 14w) \/ (s''.EX.EX_func = 15w)`
+        by fs [agp32_EX_opc_implies_EX_func] >>
+      fs [EX_ALU_update_def,Rel_def]) >-
+     (PairCases_on `p` >> rw [Run_def,dfn'Shift_def,incPC_def] >>
+      `opc ai = 1w` by fs [ag32_Decode_Shift_opc_1w] >>
+      `(s''.EX.EX_func = 9w) \/ (s''.EX.EX_func = 12w) \/ (s''.EX.EX_func = 13w) \/
+      (s''.EX.EX_func = 14w) \/ (s''.EX.EX_func = 15w)`
+        by fs [agp32_EX_opc_implies_EX_func] >>
+      fs [EX_ALU_update_def,Rel_def]) >-
+     (PairCases_on `p` >> rw [Run_def,dfn'StoreMEM_def,incPC_def] >>
+      `opc ai = 2w` by fs [ag32_Decode_StoreMEM_opc_2w] >>
+      `(s''.EX.EX_func = 9w) \/ (s''.EX.EX_func = 12w) \/ (s''.EX.EX_func = 13w) \/
+      (s''.EX.EX_func = 14w) \/ (s''.EX.EX_func = 15w)`
+        by fs [agp32_EX_opc_implies_EX_func] >>
+      fs [EX_ALU_update_def,Rel_def]) >>
+    PairCases_on `p` >> rw [Run_def,dfn'StoreMEMByte_def,incPC_def] >>
+    `opc ai = 3w` by fs [ag32_Decode_StoreMEMByte_opc_3w] >>
+    `(s''.EX.EX_func = 9w) \/ (s''.EX.EX_func = 12w) \/ (s''.EX.EX_func = 13w) \/
+    (s''.EX.EX_func = 14w) \/ (s''.EX.EX_func = 15w)`
+      by fs [agp32_EX_opc_implies_EX_func] >>
+    fs [EX_ALU_update_def,Rel_def]) >>
+  `I' (3,SUC t) = I' (3,t)` by fs [is_sch_def,is_sch_disable_def] >>
+  `~s''.ID.ID_EX_write_enable` by fs [enable_stg_def,Abbr `s`] >>
+  rw [EX_ALU_update_def] >>
+  fs [Rel_def,EX_Rel_def]
+QED
+
+
+(** EX_carry_flag and EX_overflow_flag when EX is NONE and ID is not NONE **)
+Theorem agp32_Rel_ag32_EX_ALU_flags_correct_ID_not_NONE:
+  !fext fbits a t I.
+    is_sch I (agp32 fext fbits) a ==>
+    Rel I (fext t) (agp32 fext fbits (t-1)) (agp32 fext fbits t) a t ==>
+    I (3,SUC t) = NONE ==>
+    I (2,SUC t) <> NONE ==>
+    ((agp32 fext fbits (SUC t)).EX.EX_carry_flag = (FUNPOW Next (THE (I (2,SUC t)) - 1) a).CarryFlag) /\
+    ((agp32 fext fbits (SUC t)).EX.EX_overflow_flag = (FUNPOW Next (THE (I (2,SUC t)) - 1) a).OverflowFlag)
+Proof
+  rpt gen_tac >> rpt disch_tac >>
+  `((agp32 fext fbits (SUC t)).EX.EX_carry_flag = (agp32 fext fbits t).EX.EX_carry_flag) /\
+  ((agp32 fext fbits (SUC t)).EX.EX_overflow_flag = (agp32 fext fbits t).EX.EX_overflow_flag)`
+    by METIS_TAC [agp32_Rel_EX_NONE_flags_unchanged] >>
+  fs [] >> Cases_on `enable_stg 2 (agp32 fext fbits t)` >-
+   (Cases_on `isJump_isa_op (I' (2,t)) a \/ isJump_hw_op (agp32 fext fbits t)` >-
+     (fs [is_sch_def,is_sch_decode_def] >> METIS_TAC []) >>
+    `I' (2,SUC t) = I' (1,t)` by fs [is_sch_def,is_sch_decode_def] >> fs [] >>
+    `enable_stg 3 (agp32 fext fbits t)`
+      by fs [enable_stg_def,agp32_ID_ID_write_enable_and_ID_EX_write_enable] >>
+    Cases_on `reg_data_hazard (agp32 fext fbits t)` >-
+     (fs [isJump_hw_op_def,enable_stg_def] >>
+      METIS_TAC [agp32_ID_ID_write_enable_EX_jump_sel_then_no_reg_data_hazard]) >>
+    `I' (3,SUC t) = I' (2,t)` by METIS_TAC [is_sch_def,is_sch_execute_def] >> fs [] >>
+    Cases_on `I' (3,t) <> NONE` >> fs [] >-
+     METIS_TAC [IF_EX_instr_NOT_NONE_ID_NOT_NONE] >>
+    fs [Rel_def]) >>
+  `I' (2,SUC t) = I' (2,t)` by fs [is_sch_def,is_sch_disable_def] >> fs [] >>
+  Cases_on `I' (3,t) = NONE` >-
+   fs [Rel_def] >>
+  `THE (I' (2,t)) = THE (I' (3,t)) + 1`
+    by METIS_TAC [ID_instr_index_with_EX_instr_plus_1] >> fs [Rel_def]
+QED
+
+
+(** EX_carry_flag and EX_overflow_flag when EX and ID are NONE and IF is not NONE **)
+Theorem agp32_Rel_ag32_EX_ALU_flags_correct_IF_not_NONE:
+  !fext fbits a t I.
+    is_sch I (agp32 fext fbits) a ==>
+    Rel I (fext t) (agp32 fext fbits (t-1)) (agp32 fext fbits t) a t ==>
+    I (3,SUC t) = NONE ==>
+    I (2,SUC t) = NONE ==>
+    I (1,SUC t) <> NONE ==>
+    ((agp32 fext fbits (SUC t)).EX.EX_carry_flag = (FUNPOW Next (THE (I (1,SUC t)) - 1) a).CarryFlag) /\
+    ((agp32 fext fbits (SUC t)).EX.EX_overflow_flag = (FUNPOW Next (THE (I (1,SUC t)) - 1) a).OverflowFlag)
+Proof
+  rpt gen_tac >> rpt disch_tac >>
+  `((agp32 fext fbits (SUC t)).EX.EX_carry_flag = (agp32 fext fbits t).EX.EX_carry_flag) /\
+  ((agp32 fext fbits (SUC t)).EX.EX_overflow_flag = (agp32 fext fbits t).EX.EX_overflow_flag)`
+    by METIS_TAC [agp32_Rel_EX_NONE_flags_unchanged] >>
+  fs [] >> Cases_on `enable_stg 1 (agp32 fext fbits t)` >-
+   (Cases_on `isJump_hw_op (agp32 fext fbits t)` >-
+     (`I' (1,SUC t) = SOME (THE (I' (3,t)) + 1)` by fs [is_sch_def,is_sch_fetch_def] >> fs [] >>
+      `isJump_isa_op (I' (3,t)) a` by fs [isJump_hw_op_def,Rel_def,EX_Rel_spec_def] >>
+      `I' (3,t) <> NONE` by METIS_TAC [isJump_isa_op_not_none] >>
+      fs [Rel_def]) >>
+    Cases_on `isJump_isa_op (I' (1,t)) a \/ isJump_isa_op (I' (2,t)) a \/ I' (1,t) = NONE` >-
+     (fs [is_sch_def,is_sch_fetch_def] >> METIS_TAC []) >> fs [] >>
+    `enable_stg 2 (agp32 fext fbits t)`
+      by fs [enable_stg_def,agp32_IF_PC_write_enable_and_ID_ID_write_enable] >>
+    `I' (2,SUC t) = I' (1,t)` by METIS_TAC [is_sch_def,is_sch_decode_def] >> fs []) >>
+  `~enable_stg 2 (agp32 fext fbits t)`
+    by METIS_TAC [enable_stg_def,agp32_IF_PC_write_enable_and_ID_ID_write_enable] >>
+  Cases_on `~enable_stg 3 (agp32 fext fbits t)` >> fs [] >-
+   (fs [is_sch_def,is_sch_disable_def,Rel_def] >> METIS_TAC []) >>
+  `(I' (1,SUC t) = I' (1,t)) /\ (I' (2,SUC t) = I' (2,t))`
+    by METIS_TAC [is_sch_def,is_sch_disable_def] >> fs [] >>
+  Cases_on `I' (3,t) = NONE` >-
+   fs [Rel_def] >>
+  METIS_TAC [IF_EX_instr_NOT_NONE_ID_NOT_NONE]
+QED
+
+
+(** EX_overflow_flag **)
+Theorem agp32_Rel_ag32_EX_ALU_overflow_flag_correct:
+  !fext fbits a t I.
+    is_sch I (agp32 fext fbits) a ==>
+    Rel I (fext t) (agp32 fext fbits (t-1)) (agp32 fext fbits t) a t ==>
+    I (3,SUC t) <> NONE ==>
+    (agp32 fext fbits (SUC t)).EX.EX_overflow_flag = (FUNPOW Next (THE (I (3,SUC t))) a).OverflowFlag
+Proof
+  rw [] >> Q.ABBREV_TAC `s = agp32 fext fbits t` >>
+  Q.ABBREV_TAC `s' = procs [agp32_next_state;WB_pipeline;MEM_pipeline;EX_pipeline;
+                            REG_write;ID_pipeline;IF_PC_update;Acc_compute] (fext t) s s` >>
+  Q.ABBREV_TAC `s'' = procs [IF_instr_update;ID_opc_func_update;ID_imm_update;ID_data_update;
+                             ID_data_check_update;EX_ctrl_update;EX_ALU_input_imm_update] (fext (SUC t)) s' s'` >>
+  `(agp32 fext fbits (SUC t)).EX.EX_overflow_flag = (EX_ALU_update (fext (SUC t)) s' s'').EX.EX_overflow_flag`
+    by fs [agp32_EX_ALU_items_updated_by_EX_ALU_update] >>
+  `(s''.ID.ID_EX_write_enable = s.ID.ID_EX_write_enable) /\
+  (s''.EX.EX_overflow_flag = s.EX.EX_overflow_flag) /\
+  (s''.EX.EX_carry_flag = s.EX.EX_carry_flag) /\
+  (s''.EX.EX_ALU_res = s.EX.EX_ALU_res)`
+    by METIS_TAC [agp32_same_items_until_EX_ALU_update,Abbr `s`,Abbr `s'`,Abbr `s''`] >>
+  `(s''.EX.EX_ALU_input1 = (agp32 fext fbits (SUC t)).EX.EX_ALU_input1) /\
+  (s''.EX.EX_ALU_input2 = (agp32 fext fbits (SUC t)).EX.EX_ALU_input2) /\
+  (s''.EX.EX_func = (agp32 fext fbits (SUC t)).EX.EX_func) /\
+  (s''.EX.EX_opc = (agp32 fext fbits (SUC t)).EX.EX_opc)`
+    by METIS_TAC [agp32_same_EX_ALU_input_until_ALU_update,agp32_same_EX_opc_func_until_ALU_update,
+                  Abbr `s`,Abbr `s'`,Abbr `s''`] >>
+  Cases_on `enable_stg 3 (agp32 fext fbits t)` >-
+   (`s''.ID.ID_EX_write_enable` by fs [enable_stg_def,Abbr `s`] >>
+    `s''.EX.EX_func = func (FUNPOW Next (THE (I' (3,SUC t)) − 1) a)`
+      by fs [is_sch_def,agp32_Rel_ag32_EX_func_correct] >>
+    `s''.EX.EX_opc = opc (FUNPOW Next (THE (I' (3,SUC t)) − 1) a)`
+      by fs [is_sch_def,agp32_Rel_ag32_EX_opc_correct] >>
+    `s''.EX.EX_ALU_input1 = ALU_input1 (FUNPOW Next (THE (I' (3,SUC t)) − 1) a)`
+      by fs [is_sch_def,agp32_Rel_ag32_EX_ALU_input1_correct] >>
+    `s''.EX.EX_ALU_input2 = ALU_input2 (FUNPOW Next (THE (I' (3,SUC t)) − 1) a)`
+      by fs [is_sch_def,agp32_Rel_ag32_EX_ALU_input2_correct] >>
+    Cases_on `I' (3,t) <> NONE` >-
+     (`THE (I' (3,SUC t)) = SUC (THE (I' (3,t)))`
+        by METIS_TAC [EX_instr_index_t_SUC_t_enable,ADD1] >> fs [FUNPOW_SUC] >>
+      Q.ABBREV_TAC `ai = FUNPOW Next (THE (I' (3,t))) a` >>
+      rw [Next_def,GSYM word_at_addr_def,GSYM align_addr_def] >>
+      Cases_on `Decode (word_at_addr ai.MEM (align_addr ai.PC))` >-
+       (PairCases_on `p` >> rw [Run_def,dfn'Accelerator_def,incPC_def] >>
+        `opc ai = 8w` by fs [ag32_Decode_Acc_opc_8w] >>
+        `(s''.EX.EX_func = 9w) \/ (s''.EX.EX_func = 12w) \/ (s''.EX.EX_func = 13w) \/
+        (s''.EX.EX_func = 14w) \/ (s''.EX.EX_func = 15w)`
+          by fs [agp32_EX_opc_implies_EX_func] >>
+        fs [EX_ALU_update_def,Rel_def]) >-
+       (rw [Run_def,dfn'In_def,incPC_def] >>
+        `opc ai = 7w` by fs [ag32_Decode_In_opc_7w] >>
+        `(s''.EX.EX_func = 9w) \/ (s''.EX.EX_func = 12w) \/ (s''.EX.EX_func = 13w) \/
+        (s''.EX.EX_func = 14w) \/ (s''.EX.EX_func = 15w)`
+          by fs [agp32_EX_opc_implies_EX_func] >>
+        fs [EX_ALU_update_def,Rel_def]) >-
+       (rw [Run_def,dfn'Interrupt_def,incPC_def] >>
+        `opc ai = 12w` by fs [ag32_Decode_Interrupt_opc_12w] >>
+        `(s''.EX.EX_func = 9w) \/ (s''.EX.EX_func = 12w) \/ (s''.EX.EX_func = 13w) \/
+        (s''.EX.EX_func = 14w) \/ (s''.EX.EX_func = 15w)`
+          by fs [agp32_EX_opc_implies_EX_func] >>
+        fs [EX_ALU_update_def,Rel_def]) >-
+       (PairCases_on `p` >> rw [Run_def,dfn'Jump_def] >>
+        `opc ai = 9w` by fs [ag32_Decode_Jump_opc_9w] >>
+        pairarg_tac >> fs [] >>
+        Cases_on `p0 = fAdd` >-
+         (fs [ALU_def] >> rw [] >>
+          `func ai = 0w` by fs [ag32_Decode_Jump_fAdd_func_0w] >> fs [] >>
+          rw [EX_ALU_update_def] >>
+          fs [ALU_input1_def,ALU_input2_def] >>
+          `dataA ai = ri2word p2 ai` by fs [ag32_Decode_Jump_dataA] >>
+          `ri2word p2 ai = (agp32 fext fbits (SUC t)).EX.EX_ALU_input2` by fs [] >>
+          rw [integer_wordTheory.overflow,word_msb] >> BBLAST_TAC) >>
+        Cases_on `p0 = fAddWithCarry` >-
+         (fs [ALU_def] >> rw [] >>
+          `func ai = 1w` by fs [ag32_Decode_Jump_fAddWithCarry_func_1w] >> fs [] >>
+          fs [EX_ALU_update_def,Rel_def]) >>
+        Cases_on `p0 = fSub` >-
+         (fs [ALU_def] >> rw [] >>
+          `func ai = 2w` by fs [ag32_Decode_Jump_fSub_func_2w] >> fs [] >>
+          rw [EX_ALU_update_def] >>
+          fs [ALU_input1_def,ALU_input2_def] >>
+          `dataA ai = ri2word p2 ai` by fs [ag32_Decode_Jump_dataA] >>
+          `ri2word p2 ai = (agp32 fext fbits (SUC t)).EX.EX_ALU_input2` by fs [] >> fs [] >>
+          Q.ABBREV_TAC `da = (agp32 fext fbits (SUC t)).EX.EX_ALU_input1` >>
+          Q.ABBREV_TAC `db = (agp32 fext fbits (SUC t)).EX.EX_ALU_input2` >>
+          `da + -1w * db = da - db` by WORD_DECIDE_TAC >>
+          pop_assum (fn th => rewrite_tac [th]) >>
+          rewrite_tac [integer_wordTheory.sub_overflow,word_msb] >> BBLAST_TAC) >>
+        fs [] >> rename1 `(v,ai')` >>
+        `ai'.OverflowFlag = ai.OverflowFlag` by (fs [ALU_def] >> Cases_on `p0` >> fs [] >> rw []) >>
+        `(func ai <> 0w) /\ (func ai <> 1w) /\ (func ai <> 2w)`
+          by fs [ag32_Decode_Jump_func_not_0w_1w_2w] >>
+        fs [EX_ALU_update_def,Rel_def] >>
+        Cases_on_word_value `(agp32 fext fbits (SUC t)).EX.EX_func` >> fs []) >-
+       (PairCases_on `p` >> rw [Run_def,dfn'JumpIfNotZero_def] >>
+        `opc ai = 11w` by fs [ag32_Decode_JumpIfNotZero_opc_11w] >>
+        pairarg_tac >> fs [] >>
+        Cases_on `p0 = fAdd` >-
+         (fs [ALU_def] >> rw [] >>
+          `func ai = 0w` by fs [ag32_Decode_JumpIfNotZero_fAdd_func_0w] >> fs [] >>
+          rw [EX_ALU_update_def] >>
+          fs [ALU_input1_def,ALU_input2_def] >>
+          `(dataA ai = ri2word p2 ai) /\ (dataB ai = ri2word p3 ai)`
+            by fs [ag32_Decode_JumpIfNotZero_dataA,ag32_Decode_JumpIfNotZero_dataB] >>
+          `ri2word p2 ai = (agp32 fext fbits (SUC t)).EX.EX_ALU_input1 /\
+          ri2word p3 ai = (agp32 fext fbits (SUC t)).EX.EX_ALU_input2` by fs [] >-
+           (rw [integer_wordTheory.overflow,word_msb] >> BBLAST_TAC) >>
+          rw [incPC_def] >>
+          Q.ABBREV_TAC `da = (agp32 fext fbits (SUC t)).EX.EX_ALU_input1` >>
+          Q.ABBREV_TAC `db = (agp32 fext fbits (SUC t)).EX.EX_ALU_input2` >>
+          `0w = da + db` by fs [] >>
+          pop_assum (fn th => rewrite_tac [th]) >>
+          rewrite_tac [overflow_rewrite,word_msb] >> BBLAST_TAC) >>
+        Cases_on `p0 = fAddWithCarry` >-
+         (fs [ALU_def] >> rw [incPC_def] >>
+          `func ai = 1w` by fs [ag32_Decode_JumpIfNotZero_fAddWithCarry_func_1w] >> fs [] >>
+          fs [EX_ALU_update_def,Rel_def]) >>
+        Cases_on `p0 = fSub` >-
+         (fs [ALU_def] >> rw [] >>
+          `func ai = 2w` by fs [ag32_Decode_JumpIfNotZero_fSub_func_2w] >> fs [] >>
+          rw [EX_ALU_update_def,incPC_def] >>
+          fs [ALU_input1_def,ALU_input2_def] >>
+          `(dataA ai = ri2word p2 ai) /\ (dataB ai = ri2word p3 ai)`
+            by fs [ag32_Decode_JumpIfNotZero_dataA,ag32_Decode_JumpIfNotZero_dataB] >>
+          `ri2word p2 ai = (agp32 fext fbits (SUC t)).EX.EX_ALU_input1 /\
+          ri2word p3 ai = (agp32 fext fbits (SUC t)).EX.EX_ALU_input2` by fs [] >> fs [] >>
+          Q.ABBREV_TAC `da = (agp32 fext fbits (SUC t)).EX.EX_ALU_input1` >>
+          Q.ABBREV_TAC `db = (agp32 fext fbits (SUC t)).EX.EX_ALU_input2` >-
+           (`da + -1w * db = da - db` by WORD_DECIDE_TAC >>
+            pop_assum (fn th => rewrite_tac [th]) >>
+            rewrite_tac [integer_wordTheory.sub_overflow,word_msb] >> BBLAST_TAC) >>
+          `0w = da - db` by fs [] >>
+          pop_assum (fn th => rewrite_tac [th]) >>
+          simp [sub_overflow_rewrite,word_msb]) >>
+        fs [] >> rename1 `(v,ai')` >>
+        `ai'.OverflowFlag = ai.OverflowFlag` by (fs [ALU_def] >> Cases_on `p0` >> fs [] >> rw []) >>
+        `(func ai <> 0w) /\ (func ai <> 1w) /\ (func ai <> 2w)`
+          by fs [ag32_Decode_JumpIfNotZero_func_not_0w_1w_2w] >>
+        Cases_on `v` >> rw [incPC_def] >>
+        fs [EX_ALU_update_def,Rel_def] >>
+        Cases_on_word_value `(agp32 fext fbits (SUC t)).EX.EX_func` >> fs []) >-  
+       (PairCases_on `p` >> rw [Run_def,dfn'JumpIfZero_def] >>
+        `opc ai = 10w` by fs [ag32_Decode_JumpIfZero_opc_10w] >>
+        pairarg_tac >> fs [] >>
+        Cases_on `p0 = fAdd` >-
+         (fs [ALU_def] >> rw [] >>
+          `func ai = 0w` by fs [ag32_Decode_JumpIfZero_fAdd_func_0w] >> fs [] >>
+          rw [EX_ALU_update_def] >>
+          fs [ALU_input1_def,ALU_input2_def] >>
+          `(dataA ai = ri2word p2 ai) /\ (dataB ai = ri2word p3 ai)`
+            by fs [ag32_Decode_JumpIfZero_dataA,ag32_Decode_JumpIfZero_dataB] >>
+          `ri2word p2 ai = (agp32 fext fbits (SUC t)).EX.EX_ALU_input1 /\
+          ri2word p3 ai = (agp32 fext fbits (SUC t)).EX.EX_ALU_input2` by fs [] >-
+           (fs [] >> Q.ABBREV_TAC `da = (agp32 fext fbits (SUC t)).EX.EX_ALU_input1` >>
+            Q.ABBREV_TAC `db = (agp32 fext fbits (SUC t)).EX.EX_ALU_input2` >>              
+            `0w = da + db` by fs [] >>     
+            pop_assum (fn th => rewrite_tac [th]) >>
+            rewrite_tac [overflow_rewrite,word_msb] >> BBLAST_TAC) >>
+          rw [integer_wordTheory.overflow,word_msb,incPC_def] >> BBLAST_TAC) >>
+        Cases_on `p0 = fAddWithCarry` >-
+         (fs [ALU_def] >> rw [incPC_def] >>
+          `func ai = 1w` by fs [ag32_Decode_JumpIfZero_fAddWithCarry_func_1w] >> fs [] >>
+          fs [EX_ALU_update_def,Rel_def]) >>
+        Cases_on `p0 = fSub` >-
+         (fs [ALU_def] >> rw [] >>
+          `func ai = 2w` by fs [ag32_Decode_JumpIfZero_fSub_func_2w] >> fs [] >>
+          rw [EX_ALU_update_def,incPC_def] >>
+          fs [ALU_input1_def,ALU_input2_def] >>
+          `(dataA ai = ri2word p2 ai) /\ (dataB ai = ri2word p3 ai)`
+            by fs [ag32_Decode_JumpIfZero_dataA,ag32_Decode_JumpIfZero_dataB] >>
+          `ri2word p2 ai = (agp32 fext fbits (SUC t)).EX.EX_ALU_input1 /\
+          ri2word p3 ai = (agp32 fext fbits (SUC t)).EX.EX_ALU_input2` by fs [] >> fs [] >>
+          Q.ABBREV_TAC `da = (agp32 fext fbits (SUC t)).EX.EX_ALU_input1` >>
+          Q.ABBREV_TAC `db = (agp32 fext fbits (SUC t)).EX.EX_ALU_input2` >-
+           (`0w = da - db` by fs [] >>
+            pop_assum (fn th => rewrite_tac [th]) >>
+            simp [sub_overflow_rewrite,word_msb]) >>
+          `da + -1w * db = da - db` by WORD_DECIDE_TAC >>
+          pop_assum (fn th => rewrite_tac [th]) >>
+          rewrite_tac [integer_wordTheory.sub_overflow,word_msb] >> BBLAST_TAC) >>
+        fs [] >> rename1 `(v,ai')` >>
+        `ai'.OverflowFlag = ai.OverflowFlag` by (fs [ALU_def] >> Cases_on `p0` >> fs [] >> rw []) >>
+        `(func ai <> 0w) /\ (func ai <> 1w) /\ (func ai <> 2w)`
+          by fs [ag32_Decode_JumpIfZero_func_not_0w_1w_2w] >>
+        Cases_on `v` >> rw [incPC_def] >>
+        fs [EX_ALU_update_def,Rel_def] >>
+        Cases_on_word_value `(agp32 fext fbits (SUC t)).EX.EX_func` >> fs []) >-
+       (PairCases_on `p` >> rw [Run_def,dfn'LoadConstant_def,incPC_def] >>
+        `opc ai = 13w` by fs [ag32_Decode_LoadConstant_opc_13w] >>
+        `(s''.EX.EX_func = 9w) \/ (s''.EX.EX_func = 12w) \/ (s''.EX.EX_func = 13w) \/
+        (s''.EX.EX_func = 14w) \/ (s''.EX.EX_func = 15w)`
+          by fs [agp32_EX_opc_implies_EX_func] >>
+        fs [EX_ALU_update_def,Rel_def]) >-
+       (PairCases_on `p` >> rw [Run_def,dfn'LoadMEM_def,incPC_def] >>
+        `opc ai = 4w` by fs [ag32_Decode_LoadMEM_opc_4w] >>
+        `(s''.EX.EX_func = 9w) \/ (s''.EX.EX_func = 12w) \/ (s''.EX.EX_func = 13w) \/
+        (s''.EX.EX_func = 14w) \/ (s''.EX.EX_func = 15w)`
+          by fs [agp32_EX_opc_implies_EX_func] >>
+        fs [EX_ALU_update_def,Rel_def]) >-
+       (PairCases_on `p` >> rw [Run_def,dfn'LoadMEMByte_def,incPC_def] >>
+        `opc ai = 5w` by fs [ag32_Decode_LoadMEMByte_opc_5w] >>
+        `(s''.EX.EX_func = 9w) \/ (s''.EX.EX_func = 12w) \/ (s''.EX.EX_func = 13w) \/
+        (s''.EX.EX_func = 14w) \/ (s''.EX.EX_func = 15w)`
+          by fs [agp32_EX_opc_implies_EX_func] >>
+        fs [EX_ALU_update_def,Rel_def]) >-
+       (PairCases_on `p` >> rw [Run_def,dfn'LoadUpperConstant_def,incPC_def] >>
+        `opc ai = 14w` by fs [ag32_Decode_LoadUpperConstant_opc_14w] >>
+        `(s''.EX.EX_func = 9w) \/ (s''.EX.EX_func = 12w) \/ (s''.EX.EX_func = 13w) \/
+        (s''.EX.EX_func = 14w) \/ (s''.EX.EX_func = 15w)`
+          by fs [agp32_EX_opc_implies_EX_func] >>
+        fs [EX_ALU_update_def,Rel_def]) >-
+       (PairCases_on `p` >> rw [Run_def,dfn'Normal_def,norm_def,incPC_def] >>
+        `opc ai = 0w` by fs [ag32_Decode_Normal_opc_0w] >>
+        pairarg_tac >> fs [] >>
+        Cases_on `p0 = fAdd` >-
+         (fs [ALU_def] >> rw [] >>
+          `func ai = 0w` by fs [ag32_Decode_Normal_fAdd_func_0w] >> fs [] >>
+          rw [EX_ALU_update_def] >>
+          fs [ALU_input1_def,ALU_input2_def] >>
+          `(dataA ai = ri2word p2 ai) /\ (dataB ai = ri2word p3 ai)`
+            by fs [ag32_Decode_Normal_dataA,ag32_Decode_Normal_dataB] >>
+          `ri2word p2 ai = (agp32 fext fbits (SUC t)).EX.EX_ALU_input1 /\
+          ri2word p3 ai = (agp32 fext fbits (SUC t)).EX.EX_ALU_input2` by fs [] >> fs [] >>
+          rw [integer_wordTheory.overflow,word_msb] >> BBLAST_TAC) >>
+        Cases_on `p0 = fAddWithCarry` >-
+         (fs [ALU_def] >> rw [] >>
+          `func ai = 1w` by fs [ag32_Decode_Normal_fAddWithCarry_func_1w] >> fs [] >>
+          fs [EX_ALU_update_def,Rel_def]) >>
+        Cases_on `p0 = fSub` >-
+         (fs [ALU_def] >> rw [] >>
+          `func ai = 2w` by fs [ag32_Decode_Normal_fSub_func_2w] >> fs [] >>
+          rw [EX_ALU_update_def] >>
+          fs [ALU_input1_def,ALU_input2_def] >>
+          `(dataA ai = ri2word p2 ai) /\ (dataB ai = ri2word p3 ai)`
+            by fs [ag32_Decode_Normal_dataA,ag32_Decode_Normal_dataB] >>
+          `ri2word p2 ai = (agp32 fext fbits (SUC t)).EX.EX_ALU_input1 /\
+          ri2word p3 ai = (agp32 fext fbits (SUC t)).EX.EX_ALU_input2` by fs [] >> fs [] >>
+          Q.ABBREV_TAC `da = (agp32 fext fbits (SUC t)).EX.EX_ALU_input1` >>
+          Q.ABBREV_TAC `db = (agp32 fext fbits (SUC t)).EX.EX_ALU_input2` >>
+          `da + -1w * db = da - db` by WORD_DECIDE_TAC >>
+          pop_assum (fn th => rewrite_tac [th]) >>
+          rewrite_tac [integer_wordTheory.sub_overflow,word_msb] >> BBLAST_TAC) >>
+        fs [] >> rename1 `(v,ai')` >>
+        `ai'.OverflowFlag = ai.OverflowFlag` by (fs [ALU_def] >> Cases_on `p0` >> fs [] >> rw []) >>
+        `(func ai <> 0w) /\ (func ai <> 1w) /\ (func ai <> 2w)`
+          by fs [ag32_Decode_Normal_func_not_0w_1w_2w] >>
+        fs [EX_ALU_update_def,Rel_def] >>
+        Cases_on_word_value `(agp32 fext fbits (SUC t)).EX.EX_func` >> fs []) >-
+       (PairCases_on `p` >> rw [Run_def,dfn'Out_def,norm_def,incPC_def] >>
+        `opc ai = 6w` by fs [ag32_Decode_Out_opc_6w] >>
+        pairarg_tac >> fs [] >>
+        Cases_on `p0 = fAdd` >-
+         (fs [ALU_def] >> rw [] >>
+          `func ai = 0w` by fs [ag32_Decode_Out_fAdd_func_0w] >> fs [] >>
+          rw [EX_ALU_update_def] >>
+          fs [ALU_input1_def,ALU_input2_def] >>
+          `(dataA ai = ri2word p2 ai) /\ (dataB ai = ri2word p3 ai)`
+            by fs [ag32_Decode_Out_dataA,ag32_Decode_Out_dataB] >>
+          `ri2word p2 ai = (agp32 fext fbits (SUC t)).EX.EX_ALU_input1 /\
+          ri2word p3 ai = (agp32 fext fbits (SUC t)).EX.EX_ALU_input2` by fs [] >> fs [] >>
+          rw [integer_wordTheory.overflow,word_msb] >> BBLAST_TAC) >>
+        Cases_on `p0 = fAddWithCarry` >-
+         (fs [ALU_def] >> rw [] >>
+          `func ai = 1w` by fs [ag32_Decode_Out_fAddWithCarry_func_1w] >> fs [] >>
+          fs [EX_ALU_update_def,Rel_def]) >>
+        Cases_on `p0 = fSub` >-
+         (fs [ALU_def] >> rw [] >>
+          `func ai = 2w` by fs [ag32_Decode_Out_fSub_func_2w] >> fs [] >>
+          rw [EX_ALU_update_def] >>
+          fs [ALU_input1_def,ALU_input2_def] >>
+          `(dataA ai = ri2word p2 ai) /\ (dataB ai = ri2word p3 ai)`
+            by fs [ag32_Decode_Out_dataA,ag32_Decode_Out_dataB] >>
+          `ri2word p2 ai = (agp32 fext fbits (SUC t)).EX.EX_ALU_input1 /\
+          ri2word p3 ai = (agp32 fext fbits (SUC t)).EX.EX_ALU_input2` by fs [] >> fs [] >>
+          Q.ABBREV_TAC `da = (agp32 fext fbits (SUC t)).EX.EX_ALU_input1` >>
+          Q.ABBREV_TAC `db = (agp32 fext fbits (SUC t)).EX.EX_ALU_input2` >>
+          `da + -1w * db = da - db` by WORD_DECIDE_TAC >>
+          pop_assum (fn th => rewrite_tac [th]) >>
+          rewrite_tac [integer_wordTheory.sub_overflow,word_msb] >> BBLAST_TAC) >>
+        fs [] >> rename1 `(v,ai')` >>
+        `ai'.OverflowFlag = ai.OverflowFlag` by (fs [ALU_def] >> Cases_on `p0` >> fs [] >> rw []) >>
+        `(func ai <> 0w) /\ (func ai <> 1w) /\ (func ai <> 2w)`
+          by fs [ag32_Decode_Out_func_not_0w_1w_2w] >>
+        fs [EX_ALU_update_def,Rel_def] >>
+        Cases_on_word_value `(agp32 fext fbits (SUC t)).EX.EX_func` >> fs []) >-
+       (rw [Run_def] >>
+        `opc ai = 15w` by fs [ag32_Decode_ReservedInstr_opc_15w] >>
+        `(s''.EX.EX_func = 9w) \/ (s''.EX.EX_func = 12w) \/ (s''.EX.EX_func = 13w) \/
+        (s''.EX.EX_func = 14w) \/ (s''.EX.EX_func = 15w)`
+          by fs [agp32_EX_opc_implies_EX_func] >>
+        fs [EX_ALU_update_def,Rel_def]) >-
+       (PairCases_on `p` >> rw [Run_def,dfn'Shift_def,incPC_def] >>
+        `opc ai = 1w` by fs [ag32_Decode_Shift_opc_1w] >>
+        `(s''.EX.EX_func = 9w) \/ (s''.EX.EX_func = 12w) \/ (s''.EX.EX_func = 13w) \/
+        (s''.EX.EX_func = 14w) \/ (s''.EX.EX_func = 15w)`
+          by fs [agp32_EX_opc_implies_EX_func] >>
+        fs [EX_ALU_update_def,Rel_def]) >-
+       (PairCases_on `p` >> rw [Run_def,dfn'StoreMEM_def,incPC_def] >>
+        `opc ai = 2w` by fs [ag32_Decode_StoreMEM_opc_2w] >>
+        `(s''.EX.EX_func = 9w) \/ (s''.EX.EX_func = 12w) \/ (s''.EX.EX_func = 13w) \/
+        (s''.EX.EX_func = 14w) \/ (s''.EX.EX_func = 15w)`
+          by fs [agp32_EX_opc_implies_EX_func] >>
+        fs [EX_ALU_update_def,Rel_def]) >>
+      PairCases_on `p` >> rw [Run_def,dfn'StoreMEMByte_def,incPC_def] >>
+      `opc ai = 3w` by fs [ag32_Decode_StoreMEMByte_opc_3w] >>
+      `(s''.EX.EX_func = 9w) \/ (s''.EX.EX_func = 12w) \/ (s''.EX.EX_func = 13w) \/
+      (s''.EX.EX_func = 14w) \/ (s''.EX.EX_func = 15w)`
+        by fs [agp32_EX_opc_implies_EX_func] >>
+      fs [EX_ALU_update_def,Rel_def]) >>
+    subgoal `I' (3,SUC t) = I' (2,t)` >-
+     (fs [is_sch_def,is_sch_execute_def] >>
+      Cases_on `isJump_hw_op (agp32 fext fbits t)` >>
+      Cases_on `reg_data_hazard (agp32 fext fbits t)` >>
+      METIS_TAC []) >> fs [] >>
+    `THE (I' (2,t)) = SUC (THE (I' (2,t)) - 1)`
+      by (Cases_on `THE (I' (2,t))` >- METIS_TAC [ID_instr_index_not_0] >> fs []) >>
+    `(FUNPOW Next (THE (I' (2,t))) a).OverflowFlag =
+    (FUNPOW Next (SUC (THE (I' (2,t)) - 1)) a).OverflowFlag` by METIS_TAC [] >>       
+    fs [FUNPOW_SUC] >>
+    Q.ABBREV_TAC `ai = FUNPOW Next (THE (I' (2,t)) - 1) a` >>
+    rw [Next_def,GSYM word_at_addr_def,GSYM align_addr_def] >>
+    Cases_on `Decode (word_at_addr ai.MEM (align_addr ai.PC))` >-
+     (PairCases_on `p` >> rw [Run_def,dfn'Accelerator_def,incPC_def] >>
+      `opc ai = 8w` by fs [ag32_Decode_Acc_opc_8w] >>
+      `(s''.EX.EX_func = 9w) \/ (s''.EX.EX_func = 12w) \/ (s''.EX.EX_func = 13w) \/
+      (s''.EX.EX_func = 14w) \/ (s''.EX.EX_func = 15w)`         
+        by fs [agp32_EX_opc_implies_EX_func] >>
+      fs [EX_ALU_update_def,Rel_def]) >-
+     (rw [Run_def,dfn'In_def,incPC_def] >>
+      `opc ai = 7w` by fs [ag32_Decode_In_opc_7w] >>
+      `(s''.EX.EX_func = 9w) \/ (s''.EX.EX_func = 12w) \/ (s''.EX.EX_func = 13w) \/
+      (s''.EX.EX_func = 14w) \/ (s''.EX.EX_func = 15w)`
+        by fs [agp32_EX_opc_implies_EX_func] >>
+      fs [EX_ALU_update_def,Rel_def]) >-
+     (rw [Run_def,dfn'Interrupt_def,incPC_def] >>
+      `opc ai = 12w` by fs [ag32_Decode_Interrupt_opc_12w] >>
+      `(s''.EX.EX_func = 9w) \/ (s''.EX.EX_func = 12w) \/ (s''.EX.EX_func = 13w) \/
+      (s''.EX.EX_func = 14w) \/ (s''.EX.EX_func = 15w)`
+        by fs [agp32_EX_opc_implies_EX_func] >>
+      fs [EX_ALU_update_def,Rel_def]) >-
+     (PairCases_on `p` >> rw [Run_def,dfn'Jump_def] >>
+      `opc ai = 9w` by fs [ag32_Decode_Jump_opc_9w] >>
+      pairarg_tac >> fs [] >>
+      Cases_on `p0 = fAdd` >-
+       (fs [ALU_def] >> rw [] >>
+        `func ai = 0w` by fs [ag32_Decode_Jump_fAdd_func_0w] >> fs [] >>
+        rw [EX_ALU_update_def] >>
+        fs [ALU_input1_def,ALU_input2_def] >>
+        `dataA ai = ri2word p2 ai` by fs [ag32_Decode_Jump_dataA] >>
+        `ri2word p2 ai = (agp32 fext fbits (SUC t)).EX.EX_ALU_input2` by fs [] >>
+        rw [integer_wordTheory.overflow,word_msb] >> BBLAST_TAC) >>
+      Cases_on `p0 = fAddWithCarry` >-
+       (fs [ALU_def] >> rw [] >>
+        `func ai = 1w` by fs [ag32_Decode_Jump_fAddWithCarry_func_1w] >> fs [] >>
+        fs [EX_ALU_update_def,Rel_def]) >>
+      Cases_on `p0 = fSub` >-
+       (fs [ALU_def] >> rw [] >>
+        `func ai = 2w` by fs [ag32_Decode_Jump_fSub_func_2w] >> fs [] >>
+        rw [EX_ALU_update_def] >>
+        fs [ALU_input1_def,ALU_input2_def] >>
+        `dataA ai = ri2word p2 ai` by fs [ag32_Decode_Jump_dataA] >>
+        `ri2word p2 ai = (agp32 fext fbits (SUC t)).EX.EX_ALU_input2` by fs [] >> fs [] >>
+        Q.ABBREV_TAC `da = (agp32 fext fbits (SUC t)).EX.EX_ALU_input1` >>
+        Q.ABBREV_TAC `db = (agp32 fext fbits (SUC t)).EX.EX_ALU_input2` >>
+        `da + -1w * db = da - db` by WORD_DECIDE_TAC >>
+        pop_assum (fn th => rewrite_tac [th]) >>
+        rewrite_tac [integer_wordTheory.sub_overflow,word_msb] >> BBLAST_TAC) >>
+      fs [] >> rename1 `(v,ai')` >>
+      `ai'.OverflowFlag = ai.OverflowFlag` by (fs [ALU_def] >> Cases_on `p0` >> fs [] >> rw []) >>
+      `(func ai <> 0w) /\ (func ai <> 1w) /\ (func ai <> 2w)`
+        by fs [ag32_Decode_Jump_func_not_0w_1w_2w] >>
+      fs [EX_ALU_update_def,Rel_def] >>
+      Cases_on_word_value `(agp32 fext fbits (SUC t)).EX.EX_func` >> fs []) >-
+     (PairCases_on `p` >> rw [Run_def,dfn'JumpIfNotZero_def] >>
+      `opc ai = 11w` by fs [ag32_Decode_JumpIfNotZero_opc_11w] >>
+      pairarg_tac >> fs [] >>
+      Cases_on `p0 = fAdd` >-
+       (fs [ALU_def] >> rw [] >>
+        `func ai = 0w` by fs [ag32_Decode_JumpIfNotZero_fAdd_func_0w] >> fs [] >>
+        rw [EX_ALU_update_def] >>
+        fs [ALU_input1_def,ALU_input2_def] >>
+        `(dataA ai = ri2word p2 ai) /\ (dataB ai = ri2word p3 ai)`
+          by fs [ag32_Decode_JumpIfNotZero_dataA,ag32_Decode_JumpIfNotZero_dataB] >>
+        `ri2word p2 ai = (agp32 fext fbits (SUC t)).EX.EX_ALU_input1 /\
+        ri2word p3 ai = (agp32 fext fbits (SUC t)).EX.EX_ALU_input2` by fs [] >-
+         (rw [integer_wordTheory.overflow,word_msb] >> BBLAST_TAC) >>
+        rw [incPC_def] >>
+        Q.ABBREV_TAC `da = (agp32 fext fbits (SUC t)).EX.EX_ALU_input1` >>
+        Q.ABBREV_TAC `db = (agp32 fext fbits (SUC t)).EX.EX_ALU_input2` >>
+        `0w = da + db` by fs [] >>
+        pop_assum (fn th => rewrite_tac [th]) >>
+        rewrite_tac [overflow_rewrite,word_msb] >> BBLAST_TAC) >>
+      Cases_on `p0 = fAddWithCarry` >-
+       (fs [ALU_def] >> rw [incPC_def] >>
+        `func ai = 1w` by fs [ag32_Decode_JumpIfNotZero_fAddWithCarry_func_1w] >> fs [] >>
+        fs [EX_ALU_update_def,Rel_def]) >>
+      Cases_on `p0 = fSub` >-
+       (fs [ALU_def] >> rw [] >>
+        `func ai = 2w` by fs [ag32_Decode_JumpIfNotZero_fSub_func_2w] >> fs [] >>
+        rw [EX_ALU_update_def,incPC_def] >>
+        fs [ALU_input1_def,ALU_input2_def] >>
+        `(dataA ai = ri2word p2 ai) /\ (dataB ai = ri2word p3 ai)`
+          by fs [ag32_Decode_JumpIfNotZero_dataA,ag32_Decode_JumpIfNotZero_dataB] >>
+        `ri2word p2 ai = (agp32 fext fbits (SUC t)).EX.EX_ALU_input1 /\
+        ri2word p3 ai = (agp32 fext fbits (SUC t)).EX.EX_ALU_input2` by fs [] >> fs [] >>
+        Q.ABBREV_TAC `da = (agp32 fext fbits (SUC t)).EX.EX_ALU_input1` >>
+        Q.ABBREV_TAC `db = (agp32 fext fbits (SUC t)).EX.EX_ALU_input2` >-
+         (`da + -1w * db = da - db` by WORD_DECIDE_TAC >>
+          pop_assum (fn th => rewrite_tac [th]) >>
+          rewrite_tac [integer_wordTheory.sub_overflow,word_msb] >> BBLAST_TAC) >>
+        `0w = da - db` by fs [] >>
+        pop_assum (fn th => rewrite_tac [th]) >>
+        simp [sub_overflow_rewrite,word_msb]) >>
+      fs [] >> rename1 `(v,ai')` >>
+      `ai'.OverflowFlag = ai.OverflowFlag` by (fs [ALU_def] >> Cases_on `p0` >> fs [] >> rw []) >>
+      `(func ai <> 0w) /\ (func ai <> 1w) /\ (func ai <> 2w)`
+        by fs [ag32_Decode_JumpIfNotZero_func_not_0w_1w_2w] >>
+      Cases_on `v` >> rw [incPC_def] >>
+      fs [EX_ALU_update_def,Rel_def] >>
+      Cases_on_word_value `(agp32 fext fbits (SUC t)).EX.EX_func` >> fs []) >-
+     (PairCases_on `p` >> rw [Run_def,dfn'JumpIfZero_def] >>
+      `opc ai = 10w` by fs [ag32_Decode_JumpIfZero_opc_10w] >>
+      pairarg_tac >> fs [] >>
+      Cases_on `p0 = fAdd` >-
+       (fs [ALU_def] >> rw [] >>
+        `func ai = 0w` by fs [ag32_Decode_JumpIfZero_fAdd_func_0w] >> fs [] >>
+        rw [EX_ALU_update_def] >>
+        fs [ALU_input1_def,ALU_input2_def] >>
+        `(dataA ai = ri2word p2 ai) /\ (dataB ai = ri2word p3 ai)`
+          by fs [ag32_Decode_JumpIfZero_dataA,ag32_Decode_JumpIfZero_dataB] >>
+        `ri2word p2 ai = (agp32 fext fbits (SUC t)).EX.EX_ALU_input1 /\
+        ri2word p3 ai = (agp32 fext fbits (SUC t)).EX.EX_ALU_input2` by fs [] >-
+         (fs [] >> Q.ABBREV_TAC `da = (agp32 fext fbits (SUC t)).EX.EX_ALU_input1` >>
+          Q.ABBREV_TAC `db = (agp32 fext fbits (SUC t)).EX.EX_ALU_input2` >>
+          `0w = da + db` by fs [] >>                   
+          pop_assum (fn th => rewrite_tac [th]) >>
+          rewrite_tac [overflow_rewrite,word_msb] >> BBLAST_TAC) >>
+        rw [integer_wordTheory.overflow,word_msb,incPC_def] >> BBLAST_TAC) >>
+      Cases_on `p0 = fAddWithCarry` >-
+       (fs [ALU_def] >> rw [incPC_def] >>
+        `func ai = 1w` by fs [ag32_Decode_JumpIfZero_fAddWithCarry_func_1w] >> fs [] >>
+        fs [EX_ALU_update_def,Rel_def]) >>
+      Cases_on `p0 = fSub` >-
+       (fs [ALU_def] >> rw [] >>
+        `func ai = 2w` by fs [ag32_Decode_JumpIfZero_fSub_func_2w] >> fs [] >>
+        rw [EX_ALU_update_def,incPC_def] >>
+        fs [ALU_input1_def,ALU_input2_def] >>
+        `(dataA ai = ri2word p2 ai) /\ (dataB ai = ri2word p3 ai)`
+          by fs [ag32_Decode_JumpIfZero_dataA,ag32_Decode_JumpIfZero_dataB] >>
+        `ri2word p2 ai = (agp32 fext fbits (SUC t)).EX.EX_ALU_input1 /\
+        ri2word p3 ai = (agp32 fext fbits (SUC t)).EX.EX_ALU_input2` by fs [] >> fs [] >>
+        Q.ABBREV_TAC `da = (agp32 fext fbits (SUC t)).EX.EX_ALU_input1` >>
+        Q.ABBREV_TAC `db = (agp32 fext fbits (SUC t)).EX.EX_ALU_input2` >-
+         (`0w = da - db` by fs [] >>
+          pop_assum (fn th => rewrite_tac [th]) >>
+          simp [sub_overflow_rewrite,word_msb]) >>
+        `da + -1w * db = da - db` by WORD_DECIDE_TAC >>
+        pop_assum (fn th => rewrite_tac [th]) >>
+        rewrite_tac [integer_wordTheory.sub_overflow,word_msb] >> BBLAST_TAC) >>
+      fs [] >> rename1 `(v,ai')` >>
+      `ai'.OverflowFlag = ai.OverflowFlag` by (fs [ALU_def] >> Cases_on `p0` >> fs [] >> rw []) >>
+      `(func ai <> 0w) /\ (func ai <> 1w) /\ (func ai <> 2w)`
+        by fs [ag32_Decode_JumpIfZero_func_not_0w_1w_2w] >>
+      Cases_on `v` >> rw [incPC_def] >>
+      fs [EX_ALU_update_def,Rel_def] >>
+      Cases_on_word_value `(agp32 fext fbits (SUC t)).EX.EX_func` >> fs []) >-
+     (PairCases_on `p` >> rw [Run_def,dfn'LoadConstant_def,incPC_def] >>
+      `opc ai = 13w` by fs [ag32_Decode_LoadConstant_opc_13w] >>
+      `(s''.EX.EX_func = 9w) \/ (s''.EX.EX_func = 12w) \/ (s''.EX.EX_func = 13w) \/
+      (s''.EX.EX_func = 14w) \/ (s''.EX.EX_func = 15w)`
+        by fs [agp32_EX_opc_implies_EX_func] >>
+      fs [EX_ALU_update_def,Rel_def]) >-
+     (PairCases_on `p` >> rw [Run_def,dfn'LoadMEM_def,incPC_def] >>
+      `opc ai = 4w` by fs [ag32_Decode_LoadMEM_opc_4w] >>
+      `(s''.EX.EX_func = 9w) \/ (s''.EX.EX_func = 12w) \/ (s''.EX.EX_func = 13w) \/
+      (s''.EX.EX_func = 14w) \/ (s''.EX.EX_func = 15w)`
+        by fs [agp32_EX_opc_implies_EX_func] >>
+      fs [EX_ALU_update_def,Rel_def]) >-
+     (PairCases_on `p` >> rw [Run_def,dfn'LoadMEMByte_def,incPC_def] >>
+      `opc ai = 5w` by fs [ag32_Decode_LoadMEMByte_opc_5w] >>
+      `(s''.EX.EX_func = 9w) \/ (s''.EX.EX_func = 12w) \/ (s''.EX.EX_func = 13w) \/
+      (s''.EX.EX_func = 14w) \/ (s''.EX.EX_func = 15w)`
+        by fs [agp32_EX_opc_implies_EX_func] >>
+      fs [EX_ALU_update_def,Rel_def]) >-
+     (PairCases_on `p` >> rw [Run_def,dfn'LoadUpperConstant_def,incPC_def] >>
+      `opc ai = 14w` by fs [ag32_Decode_LoadUpperConstant_opc_14w] >>
+      `(s''.EX.EX_func = 9w) \/ (s''.EX.EX_func = 12w) \/ (s''.EX.EX_func = 13w) \/
+      (s''.EX.EX_func = 14w) \/ (s''.EX.EX_func = 15w)`
+        by fs [agp32_EX_opc_implies_EX_func] >>
+      fs [EX_ALU_update_def,Rel_def]) >-
+     (PairCases_on `p` >> rw [Run_def,dfn'Normal_def,norm_def,incPC_def] >>
+      `opc ai = 0w` by fs [ag32_Decode_Normal_opc_0w] >>
+      pairarg_tac >> fs [] >>
+      Cases_on `p0 = fAdd` >-
+       (fs [ALU_def] >> rw [] >>
+        `func ai = 0w` by fs [ag32_Decode_Normal_fAdd_func_0w] >> fs [] >>
+        rw [EX_ALU_update_def] >>
+        fs [ALU_input1_def,ALU_input2_def] >>
+        `(dataA ai = ri2word p2 ai) /\ (dataB ai = ri2word p3 ai)`
+          by fs [ag32_Decode_Normal_dataA,ag32_Decode_Normal_dataB] >>
+        `ri2word p2 ai = (agp32 fext fbits (SUC t)).EX.EX_ALU_input1 /\
+        ri2word p3 ai = (agp32 fext fbits (SUC t)).EX.EX_ALU_input2` by fs [] >> fs [] >>
+        rw [integer_wordTheory.overflow,word_msb] >> BBLAST_TAC) >>
+      Cases_on `p0 = fAddWithCarry` >-
+       (fs [ALU_def] >> rw [] >>
+        `func ai = 1w` by fs [ag32_Decode_Normal_fAddWithCarry_func_1w] >> fs [] >>
+        fs [EX_ALU_update_def,Rel_def]) >>
+      Cases_on `p0 = fSub` >-
+       (fs [ALU_def] >> rw [] >>
+        `func ai = 2w` by fs [ag32_Decode_Normal_fSub_func_2w] >> fs [] >>
+        rw [EX_ALU_update_def] >>
+        fs [ALU_input1_def,ALU_input2_def] >>
+        `(dataA ai = ri2word p2 ai) /\ (dataB ai = ri2word p3 ai)`
+          by fs [ag32_Decode_Normal_dataA,ag32_Decode_Normal_dataB] >>
+        `ri2word p2 ai = (agp32 fext fbits (SUC t)).EX.EX_ALU_input1 /\
+        ri2word p3 ai = (agp32 fext fbits (SUC t)).EX.EX_ALU_input2` by fs [] >> fs [] >>
+        Q.ABBREV_TAC `da = (agp32 fext fbits (SUC t)).EX.EX_ALU_input1` >>
+        Q.ABBREV_TAC `db = (agp32 fext fbits (SUC t)).EX.EX_ALU_input2` >>
+        `da + -1w * db = da - db` by WORD_DECIDE_TAC >>
+        pop_assum (fn th => rewrite_tac [th]) >>
+        rewrite_tac [integer_wordTheory.sub_overflow,word_msb] >> BBLAST_TAC) >>
+      fs [] >> rename1 `(v,ai')` >>
+      `ai'.OverflowFlag = ai.OverflowFlag` by (fs [ALU_def] >> Cases_on `p0` >> fs [] >> rw []) >>
+      `(func ai <> 0w) /\ (func ai <> 1w) /\ (func ai <> 2w)`
+        by fs [ag32_Decode_Normal_func_not_0w_1w_2w] >>
+      fs [EX_ALU_update_def,Rel_def] >>
+      Cases_on_word_value `(agp32 fext fbits (SUC t)).EX.EX_func` >> fs []) >-
+     (PairCases_on `p` >> rw [Run_def,dfn'Out_def,norm_def,incPC_def] >>
+      `opc ai = 6w` by fs [ag32_Decode_Out_opc_6w] >>
+      pairarg_tac >> fs [] >>
+      Cases_on `p0 = fAdd` >-
+       (fs [ALU_def] >> rw [] >>
+        `func ai = 0w` by fs [ag32_Decode_Out_fAdd_func_0w] >> fs [] >>
+        rw [EX_ALU_update_def] >>
+        fs [ALU_input1_def,ALU_input2_def] >>
+        `(dataA ai = ri2word p2 ai) /\ (dataB ai = ri2word p3 ai)`
+          by fs [ag32_Decode_Out_dataA,ag32_Decode_Out_dataB] >>
+        `ri2word p2 ai = (agp32 fext fbits (SUC t)).EX.EX_ALU_input1 /\
+        ri2word p3 ai = (agp32 fext fbits (SUC t)).EX.EX_ALU_input2` by fs [] >> fs [] >>
+        rw [integer_wordTheory.overflow,word_msb] >> BBLAST_TAC) >>
+      Cases_on `p0 = fAddWithCarry` >-
+       (fs [ALU_def] >> rw [] >>
+        `func ai = 1w` by fs [ag32_Decode_Out_fAddWithCarry_func_1w] >> fs [] >>
+        fs [EX_ALU_update_def,Rel_def]) >>
+      Cases_on `p0 = fSub` >-
+       (fs [ALU_def] >> rw [] >>
+        `func ai = 2w` by fs [ag32_Decode_Out_fSub_func_2w] >> fs [] >>
+        rw [EX_ALU_update_def] >>
+        fs [ALU_input1_def,ALU_input2_def] >>
+        `(dataA ai = ri2word p2 ai) /\ (dataB ai = ri2word p3 ai)`
+          by fs [ag32_Decode_Out_dataA,ag32_Decode_Out_dataB] >>
+        `ri2word p2 ai = (agp32 fext fbits (SUC t)).EX.EX_ALU_input1 /\
+        ri2word p3 ai = (agp32 fext fbits (SUC t)).EX.EX_ALU_input2` by fs [] >> fs [] >>
+        Q.ABBREV_TAC `da = (agp32 fext fbits (SUC t)).EX.EX_ALU_input1` >>
+        Q.ABBREV_TAC `db = (agp32 fext fbits (SUC t)).EX.EX_ALU_input2` >>
+        `da + -1w * db = da - db` by WORD_DECIDE_TAC >>
+        pop_assum (fn th => rewrite_tac [th]) >>
+        rewrite_tac [integer_wordTheory.sub_overflow,word_msb] >> BBLAST_TAC) >>
+      fs [] >> rename1 `(v,ai')` >>
+      `ai'.OverflowFlag = ai.OverflowFlag` by (fs [ALU_def] >> Cases_on `p0` >> fs [] >> rw []) >>
+      `(func ai <> 0w) /\ (func ai <> 1w) /\ (func ai <> 2w)`
+        by fs [ag32_Decode_Out_func_not_0w_1w_2w] >>
+      fs [EX_ALU_update_def,Rel_def] >>
+      Cases_on_word_value `(agp32 fext fbits (SUC t)).EX.EX_func` >> fs []) >-
+     (rw [Run_def] >>
+      `opc ai = 15w` by fs [ag32_Decode_ReservedInstr_opc_15w] >>
+      `(s''.EX.EX_func = 9w) \/ (s''.EX.EX_func = 12w) \/ (s''.EX.EX_func = 13w) \/
+      (s''.EX.EX_func = 14w) \/ (s''.EX.EX_func = 15w)`
+        by fs [agp32_EX_opc_implies_EX_func] >>
+      fs [EX_ALU_update_def,Rel_def]) >-
+     (PairCases_on `p` >> rw [Run_def,dfn'Shift_def,incPC_def] >>
+      `opc ai = 1w` by fs [ag32_Decode_Shift_opc_1w] >>
+      `(s''.EX.EX_func = 9w) \/ (s''.EX.EX_func = 12w) \/ (s''.EX.EX_func = 13w) \/
+      (s''.EX.EX_func = 14w) \/ (s''.EX.EX_func = 15w)`
+        by fs [agp32_EX_opc_implies_EX_func] >>
+      fs [EX_ALU_update_def,Rel_def]) >-
+     (PairCases_on `p` >> rw [Run_def,dfn'StoreMEM_def,incPC_def] >>
+      `opc ai = 2w` by fs [ag32_Decode_StoreMEM_opc_2w] >>
+      `(s''.EX.EX_func = 9w) \/ (s''.EX.EX_func = 12w) \/ (s''.EX.EX_func = 13w) \/
+      (s''.EX.EX_func = 14w) \/ (s''.EX.EX_func = 15w)`
+        by fs [agp32_EX_opc_implies_EX_func] >>
+      fs [EX_ALU_update_def,Rel_def]) >>
+    PairCases_on `p` >> rw [Run_def,dfn'StoreMEMByte_def,incPC_def] >>
+    `opc ai = 3w` by fs [ag32_Decode_StoreMEMByte_opc_3w] >>
+    `(s''.EX.EX_func = 9w) \/ (s''.EX.EX_func = 12w) \/ (s''.EX.EX_func = 13w) \/
+    (s''.EX.EX_func = 14w) \/ (s''.EX.EX_func = 15w)`
+      by fs [agp32_EX_opc_implies_EX_func] >>
+    fs [EX_ALU_update_def,Rel_def]) >>
+  `I' (3,SUC t) = I' (3,t)` by fs [is_sch_def,is_sch_disable_def] >>
+  `~s''.ID.ID_EX_write_enable` by fs [enable_stg_def,Abbr `s`] >>
+  rw [EX_ALU_update_def] >>
+  fs [Rel_def,EX_Rel_def]
+QED
+
+val _ = export_theory ();
